# baseURI: http://www.w3.org/ns/sosa/oml
# imports: http://def.seegrid.csiro.au/ontology/om/om-lite
# imports: http://def.seegrid.csiro.au/ontology/om/sam-lite
# imports: http://www.w3.org/ns/sosa/
# prefix: sosa-oml

@prefix dc: <http://purl.org/dc/elements/1.1/> .
@prefix dcterms: <http://purl.org/dc/terms/> .
@prefix meta: <http://meta.schema.org/> .
@prefix oml: <http://def.seegrid.csiro.au/ontology/om/om-lite#> .
@prefix owl: <http://www.w3.org/2002/07/owl#> .
@prefix rdf: <http://www.w3.org/1999/02/22-rdf-syntax-ns#> .
@prefix rdfs: <http://www.w3.org/2000/01/rdf-schema#> .
@prefix samfl: <http://def.seegrid.csiro.au/ontology/om/sam-lite#> .
@prefix skos: <http://www.w3.org/2004/02/skos/core#> .
@prefix sosa: <http://www.w3.org/ns/sosa/> .
@prefix sosa-oml: <http://www.w3.org/ns/sosa/oml#> .
@prefix xsd: <http://www.w3.org/2001/XMLSchema#> .

oml:Observation
  owl:equivalentClass sosa:Observation ;
.
oml:Process
  owl:equivalentClass [
      rdf:type owl:Class ;
      owl:unionOf (
          sosa:Sensor
          sosa-oml:ObservationProcedure
        ) ;
    ] ;
.
oml:featureOfInterest
  owl:equivalentProperty sosa:hasFeatureOfInterest ;
.
oml:observedProperty
  owl:equivalentProperty sosa:observedProperty ;
.
oml:phenomenonTime
  owl:equivalentProperty sosa:phenomenonTime ;
.
oml:procedure
  rdfs:comment "sub-property of sosa:usedPropecedure which also covers procedures for actuation and sampling" ;
  rdfs:subPropertyOf sosa:usedProcedure ;
.
oml:result
  rdfs:comment "sub-property of sosa:hasResult which also covers actuation and sampling" ;
  rdfs:subPropertyOf sosa:hasResult ;
.
oml:resultTime
  rdfs:comment "sub-property of sosa:resultTime which also relates to actuation and sampling events" ;
  rdfs:subPropertyOf sosa:resultTime ;
.
samfl:Process
  owl:equivalentClass [
      rdf:type owl:Class ;
      owl:unionOf (
          sosa-oml:SamplingProcedure
          sosa-oml:SamplingDevice
        ) ;
    ] ;
.
samfl:SamplingFeature
  owl:equivalentClass sosa:Sample ;
.
samfl:hostedProcedure
  rdfs:comment "When a sampling feature hosts a procedure or instrument it is acting as a platform." ;
  rdfs:comment "sub-property of sosa:hosts which relates a platform to an observation, actuation or sampling procedure" ;
  rdfs:subPropertyOf sosa:hosts ;
.
samfl:sampledFeature
  owl:equivalentProperty sosa:isSampleOf ;
.
samfl:samplingMethod
  rdfs:subPropertyOf sosa:usedProcedure ;
.
samfl:samplingTime
  rdfs:comment "sub-property of sosa:resultTime which also relates to actuation and observation events" ;
  rdfs:subPropertyOf sosa:resultTime ;
.
sosa:Procedure
  owl:equivalentClass [
      rdf:type owl:Class ;
      owl:disjointUnionOf (
          sosa-oml:ActuationProcedure
          sosa-oml:ObservationProcedure
          sosa-oml:SamplingProcedure
        ) ;
    ] ;
.
sosa:hasResult
  meta:domainIncludes sosa-oml:SamplingEvent ;
.
sosa:isResultOf
  meta:rangeIncludes sosa-oml:SamplingEvent ;
  rdfs:comment "... or SamplingEvent" ;
  skos:definition "... or SamplingEvent" ;
.
sosa:oml
  rdf:type owl:Ontology ;
  dc:creator "Simon J D Cox" ;
  dcterms:created "2016-12-14" ;
  rdfs:comment """Mapping of the om-lite/sam-lite implementations of O&M with the W3C/OGC SOSA ontology. 

N.B. om-lite/sam-lite are idiomatic OWL implementations of the O&M model from ISO 19156:2011, 
documented in Semantic Web Journal, v8, n3 2017"""@en ;
  rdfs:comment "This graph is provisional. It is the work of only one person and is provided to allow evaluation and support discussion of the potential modularization approach." ;
  rdfs:label "Alignment of om-lite + sam-lite with SOSA"@en ;
  rdfs:seeAlso <http://def.seegrid.csiro.au/ontology/om/om-lite> ;
  rdfs:seeAlso <http://def.seegrid.csiro.au/ontology/om/sam-lite> ;
  rdfs:seeAlso <http://www.semantic-web-journal.net/content/ontology-observations-and-sampling-features-alignments-existing-models-0> ;
  owl:imports <http://def.seegrid.csiro.au/ontology/om/om-lite> ;
  owl:imports <http://def.seegrid.csiro.au/ontology/om/sam-lite> ;
  owl:imports sosa: ;
.
sosa-oml:ActuationProcedure
  rdf:type owl:Class ;
  rdfs:comment "(Notional) Actuation procedure or recipe, complementing SamplingProcedure and ObservationProcedure"@en ;
  rdfs:label "Actuation procedure"@en ;
  rdfs:subClassOf sosa:Procedure ;
  owl:disjointWith sosa-oml:ObservationProcedure ;
  owl:disjointWith sosa-oml:SamplingProcedure ;
.
sosa-oml:ObservationProcedure
  rdf:type owl:Class ;
  rdfs:comment "(Notional) Observation or sensing procedure or recipe, complementing SamplingProcedure and ActuationProcedure"@en ;
  rdfs:label "Observation procedure"@en ;
  rdfs:subClassOf oml:Process ;
  rdfs:subClassOf sosa:Procedure ;
  owl:disjointWith sosa-oml:ActuationProcedure ;
  owl:disjointWith sosa-oml:SamplingProcedure ;
.
sosa-oml:SamplingDevice
  rdf:type owl:Class ;
  rdfs:comment "(Notional) Sampling or sample preparation or processing device, complementing sosa:Sensor and sosa:Actuator"@en ;
  rdfs:label "Sampling device"@en ;
  rdfs:subClassOf samfl:Process ;
.
sosa-oml:SamplingEvent
  rdf:type owl:Class ;
  rdfs:comment "(Notional) Sampling or sample preparation or processing event, complementing sosa:Observation and sosa:Actuation"@en ;
  rdfs:label "Sampling event"@en ;
.
sosa-oml:SamplingProcedure
  rdf:type owl:Class ;
  rdfs:comment "(Notional) Sampling or sample preparation or processing procedure or recipe, complementing ObservationProcedure and ActuationProcedure"@en ;
  rdfs:label "Sampling procedure"@en ;
  rdfs:subClassOf samfl:Process ;
  rdfs:subClassOf sosa:Procedure ;
  owl:disjointWith sosa-oml:ActuationProcedure ;
  owl:disjointWith sosa-oml:ObservationProcedure ;
.
sosa:usedProcedure
  meta:domainIncludes sosa-oml:SamplingEvent ;
.
