@prefix : <https://github.com/w3c/omn/blob/master/omnlib/ontologies/omn-monitoring-genericconcepts#> .
@prefix dc: <http://purl.org/dc/elements/1.1/> .
@prefix owl: <http://www.w3.org/2002/07/owl#> .
@prefix rdf: <http://www.w3.org/1999/02/22-rdf-syntax-ns#> .
@prefix xml: <http://www.w3.org/XML/1998/namespace#> .
@prefix xsd: <http://www.w3.org/2001/XMLSchema#> .
@prefix rdfs: <http://www.w3.org/2000/01/rdf-schema#> .
@prefix vann: <http://purl.org/vocab/vann/> .
@prefix dcterms: <http://purl.org/dc/terms/> .
@prefix omn: <https://github.com/w3c/omn/blob/master/omnlib/ontologies/omn#> .
@prefix omn-service: <https://github.com/w3c/omn/blob/master/omnlib/ontologies/omn-service#> .
@prefix omn-resource: <https://github.com/w3c/omn/blob/master/omnlib/ontologies/omn-resource#> .
@prefix omn-component: <https://github.com/w3c/omn/blob/master/omnlib/ontologies/omn-component#> .
@prefix omn-lifecycle: <https://github.com/w3c/omn/blob/master/omnlib/ontologies/omn-lifecycle#> .
@prefix omn-federation: <https://github.com/w3c/omn/blob/master/omnlib/ontologies/omn-federation#> .
@prefix omn-monitoring: <https://github.com/w3c/omn/blob/master/omnlib/ontologies/omn-monitoring#> .
@prefix omn-monitoring-data: <https://github.com/w3c/omn/blob/master/omnlib/ontologies/omn-monitoring-data#> .
@prefix omn-monitoring-unit: <https://github.com/w3c/omn/blob/master/omnlib/ontologies/omn-monitoring-unit#> .
@prefix omn-monitoring-tool: <https://github.com/w3c/omn/blob/master/omnlib/ontologies/omn-monitoring-tool#> .
@prefix omn-monitoring-metric: <https://github.com/w3c/omn/blob/master/omnlib/ontologies/omn-monitoring-metric#> .
@base <https://github.com/w3c/omn/blob/master/omnlib/ontologies/omn-monitoring-genericconcepts> .

<https://github.com/w3c/omn/blob/master/omnlib/ontologies/omn-monitoring-genericconcepts> rdf:type owl:Ontology ;
                                                                    
                                                                    rdfs:label "omn-monitoring-genericconcepts"@en ;
                                                                    
                                                                    dc:title "Open-Multinet Monitoring GenericConcepts Ontology"^^xsd:string ;
                                                                    
                                                                    dc:description "The generic concepts ontology describes generic concepts such as measurement location, timestamp, transport protocols, etc."^^xsd:string ;
                                                                    
                                                                    vann:preferredNamespacePrefix "omn-monitoring-genericconcepts" ;
                                                                    
                                                                    vann:preferredNamespaceUri "https://github.com/w3c/omn/blob/master/omnlib/ontologies/omn-monitoring-genericconcepts#" ;
                                                                    
                                                                    dc:date "2015-05-30" ;
                                                                                                                                        
                                                                    dcterms:license <http://creativecommons.org/licenses/by/4.0/> ;
                                                                    
                                                                    dc:publisher <http://open-multinet.info/> ;
                                                                                                                                        
                                                                    dc:creator <https://www.linkedin.com/in/yahyaalhazmi> ;
                                                                    
                                                                    dc:author <https://www.linkedin.com/in/yahyaalhazmi> ;
                                                                    
                                                                    dc:contributor <http://alex.willner.ws/about#me> ;
                                                                    dc:contributor <mailto:jorge.lopez_vergara@uam.es> ;
                                                                    dc:contributor <mailto:steger@complex.elte.hu> ;
                                                                    dc:contributor <mailto:lakis@inf.elte.hu> ;
                                                                    dc:contributor <mailto:chrisap@noc.ntua.gr> ;
                                                                    dc:contributor <http://www.commit-nl.nl/people/morsey> ;
                                                                    dc:contributor <https://staff.fnwi.uva.nl/p.grosso> .
                                                                    


#################################################################
#
#    Object Properties
#
#################################################################


###  https://github.com/w3c/omn/blob/master/omnlib/ontologies/omn-monitoring-genericconcepts#locatedAt

:locatedAt rdf:type owl:ObjectProperty ;
                      
           rdfs:range :Location ;

           rdfs:domain [ rdf:type owl:Class ;
                         owl:unionOf ( omn:Service
                                       omn-monitoring:Tool
                                       omn-monitoring-data:Measurement
                                       :MonitoringDomain
                                     )
                       ] .



###  https://github.com/w3c/omn/blob/master/omnlib/ontologies/omn-monitoring-genericconcepts#usesProtocol

:usesProtocol rdf:type owl:ObjectProperty ;
                      
              rdfs:range :Protocol ;

              rdfs:domain [ rdf:type owl:Class ;
                            owl:unionOf ( omn:Service
                                          :Protocol
                                        )
                          ] .


###  https://github.com/w3c/omn/blob/master/omnlib/ontologies/omn-monitoring-genericconcepts#query

:query rdf:type owl:ObjectProperty ;
                      
       rdfs:domain omn-monitoring:Tool ;

       rdfs:range [ rdf:type owl:Class ;
                     owl:unionOf ( omn:Service
                                   omn-monitoring:Tool
                                 )
                   ] .


#################################################################
#
#    Data properties
#
#################################################################


###  https://github.com/w3c/omn/blob/master/omnlib/ontologies/omn-monitoring-genericconcepts#latitude

:latitude rdf:type owl:DatatypeProperty ;
              
          rdfs:comment "Determines the latitude coordinate of a physical location."^^xsd:string ;
              
          rdfs:domain :PhysicalLocation ;
              
          rdfs:range xsd:float .



###  https://github.com/w3c/omn/blob/master/omnlib/ontologies/omn-monitoring-genericconcepts#longitude

:longitude rdf:type owl:DatatypeProperty ;
              
           rdfs:comment "Determines the longitude coordinate of a physical location."^^xsd:string ;
              
           rdfs:domain :PhysicalLocation ;
              
           rdfs:range xsd:float .





#################################################################
#
#    Classes
#
#################################################################


###  https://github.com/w3c/omn/blob/master/omnlib/ontologies/omn-monitoring-genericconcepts#Protocol

:Protocol rdf:type owl:Class ;
          
          rdfs:comment "Represents protocols used for measurement data exchange and reporting."^^xsd:string .



###  https://github.com/w3c/omn/blob/master/omnlib/ontologies/omn-monitoring-genericconcepts#ApplicationProtocol

:ApplicationProtocol rdf:type owl:Class ;
                     
                     rdfs:subClassOf :Protocol ;
                     
                     rdfs:comment "Represents protocols used to transport data at the application level such as IPFIX, SNMP, OMSP, etc."^^xsd:string .



###  https://github.com/w3c/omn/blob/master/omnlib/ontologies/omn-monitoring-genericconcepts#TransportProtocol

:TransportProtocol rdf:type owl:Class ;
                   
                   rdfs:subClassOf :Protocol ;
                   
                   rdfs:comment "Represents protocol used by a measurement tool or framework at the transport layer, e.g. TCP, UDP, SCTP, etc."^^xsd:string .



###  https://github.com/w3c/omn/blob/master/omnlib/ontologies/omn-monitoring-genericconcepts#AuthenticationMethod

:AuthenticationMethod rdf:type owl:Class ;
                      
                      rdfs:comment "Represents the method used for authentications in order to either read or write data."^^xsd:string .



###  https://github.com/w3c/omn/blob/master/omnlib/ontologies/omn-monitoring-genericconcepts#Event

:Event rdf:type owl:Class ;
       
       rdfs:comment "Represents any event or notification within a system during processing phase, e.g CPU load is over a defined threshold, a resource is created or deleted, etc.."^^xsd:string .



###  https://github.com/w3c/omn/blob/master/omnlib/ontologies/omn-monitoring-genericconcepts#Location

:Location rdf:type owl:Class ;
          
          rdfs:comment "Represents location of monitoring and measurement related concepts, such as location measurements (i.e. measured metric), data collectors, etc."^^xsd:string .



###  https://github.com/w3c/omn/blob/master/omnlib/ontologies/omn-monitoring-genericconcepts#LogicalLocation

:LogicalLocation rdf:type owl:Class ;
                 
                 rdfs:subClassOf :Location ;
                 
                 rdfs:comment "Represents logical location, (e.g. URI) of FTPservice, SPARQLEndpoint, SQLServer, WebResource, Webservice (REST, SOAP, SQREME), collectionEndpoint."^^xsd:string .



###  https://github.com/w3c/omn/blob/master/omnlib/ontologies/omn-monitoring-genericconcepts#PhysicalLocation

:PhysicalLocation rdf:type owl:Class ;
                  
                  rdfs:subClassOf :Location ;
                  
                  rdfs:comment "Represents physical location."^^xsd:string .



###  https://github.com/w3c/omn/blob/master/omnlib/ontologies/omn-monitoring-genericconcepts#MonitoringDomain

:MonitoringDomain rdf:type owl:Class ;
                  
                  rdfs:subClassOf omn-federation:Infrastructure ;

                  rdfs:comment "Represents the domain or the area that is being monitored."^^xsd:string .



###  https://github.com/w3c/omn/blob/master/omnlib/ontologies/omn-monitoring-genericconcepts#Query

:Query rdf:type owl:Class ;

       rdfs:subClassOf omn-lifecycle:Request ;
       
       rdfs:comment "Represents queries used to retrieve data."^^xsd:string .



###  https://github.com/w3c/omn/blob/master/omnlib/ontologies/omn-monitoring-genericconcepts#SingleQuery

:SingleQuery rdf:type owl:Class ;

             rdfs:subClassOf :Query ;
       
             rdfs:comment "Represents one single query to retrieve data about particular metric of one or more resources."^^xsd:string .



###  https://github.com/w3c/omn/blob/master/omnlib/ontologies/omn-monitoring-genericconcepts#BatchQuery

:BatchQuery rdf:type owl:Class ;
       
       rdfs:comment "Represents batch of queries to retrieve data about multiple metrics of multiple resources."^^xsd:string .



###  https://github.com/w3c/omn/blob/master/omnlib/ontologies/omn-monitoring-genericconcepts#ConditionalNotSatisfiedEvent

:ConditionalNotSatisfiedEvent rdf:type owl:Class ;
                                              
                              rdfs:subClassOf :Event ;

                              rdfs:comment "Represents an event that occurs if a condition is not satisified."^^xsd:string .



###  https://github.com/w3c/omn/blob/master/omnlib/ontologies/omn-monitoring-genericconcepts#EventAtMeasurementPhase

:EventAtMeasurementPhase rdf:type owl:Class ;
                                              
                         rdfs:subClassOf :Event ;

                         rdfs:comment "Represents an event that occurs during a measurement phase."^^xsd:string .



###  https://github.com/w3c/omn/blob/master/omnlib/ontologies/omn-monitoring-genericconcepts#ToolUnavailableEvent

:ToolUnavailableEvent rdf:type owl:Class ;
                                              
                      rdfs:subClassOf :EventAtMeasurementPhase ;

                      rdfs:comment "Represents an event that occurs if a contacted tool is not available."^^xsd:string .



###  https://github.com/w3c/omn/blob/master/omnlib/ontologies/omn-monitoring-genericconcepts#NoToolConfiguredToMeasureMetric

:NoToolConfiguredToMeasureMetric rdf:type owl:Class ;
                                              
                                 rdfs:subClassOf :EventAtMeasurementPhase ;

                                 rdfs:comment "Represents an event that occurs if there is no tool is configured to measure the concered metric(s)."^^xsd:string .





#################################################################
#
#    Individuals
#
#################################################################



###  https://github.com/w3c/omn/blob/master/omnlib/ontologies/omn-monitoring-genericconcepts#OMSP

:OMSP rdf:type :ApplicationProtocol ,
               owl:NamedIndividual ;
                                          
      rdfs:comment "The OML Measurement Stream Protocol (OMSP) is used by the Orbit Measurement Library (OML) to describe and transport measurement tuples between injection points (OML clients) and processing/collection points (OML servers)."^^xsd:string .



##  https://github.com/w3c/omn/blob/master/omnlib/ontologies/omn-monitoring-genericconcepts#SNMP

:SNMP rdf:type :ApplicationProtocol ,
               owl:NamedIndividual ;
                     
      rdfs:comment "The Simple Network Management Protocol (SNMP) that is used within the OML framework for transfering the data between the OML clients and server."^^xsd:string .



##  https://github.com/w3c/omn/blob/master/omnlib/ontologies/omn-monitoring-genericconcepts#IPFIX

:IPFIX rdf:type :ApplicationProtocol ,
                owl:NamedIndividual ;
                     
       rdfs:comment "IPFIX protocol is used to export IP traffic flow information over the network."^^xsd:string .



###  https://github.com/w3c/omn/blob/master/omnlib/ontologies/omn-monitoring-genericconcepts#TCP

:TCP rdf:type :TransportProtocol ,
               owl:NamedIndividual ;

     rdfs:comment "The Transmission Control Protocol (TCP) is a transport-layer protocol, which is one of the core members of the Internet protocol suite."^^xsd:string .



###  https://github.com/w3c/omn/blob/master/omnlib/ontologies/omn-monitoring-genericconcepts#UDP

:UDP rdf:type :TransportProtocol ,
               owl:NamedIndividual ;

     rdfs:comment "The User Datagram Protocol (UDP) is a transport-layer protocol, which is one of the core members of the Internet protocol suite."^^xsd:string .



###  https://github.com/w3c/omn/blob/master/omnlib/ontologies/omn-monitoring-genericconcepts#SCTP

:SCTP rdf:type :TransportProtocol ,
               owl:NamedIndividual ;

      rdfs:comment "The Stream Control Transmission Protocol (SCTP) is a transport-layer protocol. It serves similar to the Transmission Control Protocol (TCP) and User Datagram Protocol (UDP). It provides some of the same features of UDP and TCP, it is message-oriented like UDP and ensures reliable, in-sequence transport of messages with congestion control like TCP. SCTP specification @https://tools.ietf.org/html/rfc6525"^^xsd:string .



###  Generated by the OWL API (version 3.5.1) http://owlapi.sourceforge.net

