@prefix v3-ExposureMode: <http://hl7.org/fhir/v3/ExposureMode/> .
@prefix fhir:  <http://hl7.org/fhir/> .
@prefix rdf:   <http://www.w3.org/1999/02/22-rdf-syntax-ns#> .
@prefix owl:   <http://www.w3.org/2002/07/owl#> .
@prefix xsd:   <http://www.w3.org/2001/XMLSchema#> .
@prefix skos:  <http://www.w3.org/2004/02/skos/core#> .
@prefix rdfs:  <http://www.w3.org/2000/01/rdf-schema#> .
@prefix w5:    <http://hl7.org/fhir/w5#> .

v3-ExposureMode:AIRBORNE
        a                owl:Class ;
        rdfs:label       "airborne" ;
        rdfs:subClassOf  v3-ExposureMode:_ExposureMode ;
        skos:definition  "Description: Communication of an agent from a living subject or environmental source to a living subject through indirect contact via oral or nasal inhalation." ;
        skos:prefLabel   "airborne" .

v3-ExposureMode:WATERBORNE
        a                owl:Class ;
        rdfs:label       "waterborne" ;
        rdfs:subClassOf  v3-ExposureMode:_ExposureMode ;
        skos:definition  "Description: Communication of an agent to a living subject by contact and/or consumption via an aqueous medium" ;
        skos:prefLabel   "waterborne" .

v3-ExposureMode:_ExposureMode
        a                owl:Class ;
        rdfs:label       "ExposureMode" ;
        skos:definition  "Code for the mechanism by which the exposure agent was exchanged or potentially exchanged by the participants involved in the exposure." ;
        skos:prefLabel   "ExposureMode" .

v3-ExposureMode:CONTACT
        a                owl:Class ;
        rdfs:label       "contact" ;
        rdfs:subClassOf  v3-ExposureMode:_ExposureMode ;
        skos:definition  "Description: Communication of an agent from a living subject or environmental source to a living subject through direct physical contact." ;
        skos:prefLabel   "contact" .

v3-ExposureMode:  a      owl:Ontology ;
        rdfs:comment     " Code for the mechanism by which the exposure agent was exchanged or potentially exchanged by the participants involved in the exposure." ;
        rdfs:label       "v3 Code System ExposureMode" ;
        owl:versionIRI   "http://hl7.org/fhir/v3/ExposureMode/2016-11-11" ;
        owl:versionInfo  "v3 Code System ExposureMode(2016-11-11)" .

v3-ExposureMode:FOODBORNE
        a                owl:Class ;
        rdfs:label       "foodborne" ;
        rdfs:subClassOf  v3-ExposureMode:_ExposureMode ;
        skos:definition  "Description: Communication of an agent from a food source to a living subject via oral consumption." ;
        skos:prefLabel   "foodborne" .
