@prefix v3-hl7Realm: <http://hl7.org/fhir/v3/hl7Realm/> .
@prefix fhir:  <http://hl7.org/fhir/> .
@prefix rdf:   <http://www.w3.org/1999/02/22-rdf-syntax-ns#> .
@prefix owl:   <http://www.w3.org/2002/07/owl#> .
@prefix xsd:   <http://www.w3.org/2001/XMLSchema#> .
@prefix skos:  <http://www.w3.org/2004/02/skos/core#> .
@prefix rdfs:  <http://www.w3.org/2000/01/rdf-schema#> .
@prefix w5:    <http://hl7.org/fhir/w5#> .

v3-hl7Realm:CO  a        owl:Class ;
        rdfs:label       "Columbia" ;
        rdfs:subClassOf  v3-hl7Realm:AffiliateRealms ;
        skos:definition  "Description: Realm code for use of Localized Version" ;
        skos:prefLabel   "Columbia" .

v3-hl7Realm:AT  a        owl:Class ;
        rdfs:label       "Austria" ;
        rdfs:subClassOf  v3-hl7Realm:AffiliateRealms ;
        skos:definition  "Description: Realm code for use of Austria" ;
        skos:prefLabel   "Austria" .

v3-hl7Realm:IE  a        owl:Class ;
        rdfs:label       "Ireland" ;
        rdfs:subClassOf  v3-hl7Realm:AffiliateRealms ;
        skos:definition  "Description: Realm code for use of Ireland" ;
        skos:prefLabel   "Ireland" .

v3-hl7Realm:LT  a        owl:Class ;
        rdfs:label       "Lithuania" ;
        rdfs:subClassOf  v3-hl7Realm:AffiliateRealms ;
        skos:definition  "Description: Realm code for use of Lithuania" ;
        skos:prefLabel   "Lithuania" .

v3-hl7Realm:CZ  a        owl:Class ;
        rdfs:label       "Czech Republic" ;
        rdfs:subClassOf  v3-hl7Realm:AffiliateRealms ;
        skos:definition  "Description: Realm code for use of Czech Republic" ;
        skos:prefLabel   "Czech Republic" .

v3-hl7Realm:NZ  a        owl:Class ;
        rdfs:label       "New Zealand" ;
        rdfs:subClassOf  v3-hl7Realm:AffiliateRealms ;
        skos:definition  "Description: Realm code for use of New Zealand" ;
        skos:prefLabel   "New Zealand" .

v3-hl7Realm:UY  a        owl:Class ;
        rdfs:label       "Uruguay" ;
        rdfs:subClassOf  v3-hl7Realm:AffiliateRealms ;
        skos:definition  "Description: Realm code for use of Uruguay" ;
        skos:prefLabel   "Uruguay" .

v3-hl7Realm:AffiliateRealms
        a                owl:Class ;
        rdfs:label       "Affiliate Realms" ;
        rdfs:subClassOf  v3-hl7Realm:BindingRealms ;
        skos:definition  "Description: Realm codes for official HL7 organizational bodies.  This includes both the HL7 International organization as well as all recognized international affiliates (past and present).  These groups have the ability to bind vocabulary and develop artifacts.  As well, they have the ability to have \"ownership\" over other binding realms and namespace realms via the owningAffiliate property of those other realm codes." ;
        skos:prefLabel   "Affiliate Realms" .

v3-hl7Realm:FR  a        owl:Class ;
        rdfs:label       "France" ;
        rdfs:subClassOf  v3-hl7Realm:AffiliateRealms ;
        skos:definition  "Description: Realm code for use of France" ;
        skos:prefLabel   "France" .

v3-hl7Realm:US  a        owl:Class ;
        rdfs:label       "United States of America" ;
        rdfs:subClassOf  v3-hl7Realm:AffiliateRealms ;
        skos:definition  "Description: Realm code for use of United States of America" ;
        skos:prefLabel   "United States of America" .

v3-hl7Realm:RU  a        owl:Class ;
        rdfs:label       "Russian Federation" ;
        rdfs:subClassOf  v3-hl7Realm:AffiliateRealms ;
        skos:definition  "Description: Realm code for use of Russian Federation" ;
        skos:prefLabel   "Russian Federation" .

v3-hl7Realm:SG  a        owl:Class ;
        rdfs:label       "Singapore" ;
        rdfs:subClassOf  v3-hl7Realm:AffiliateRealms ;
        skos:definition  "Description: Realm code for use of Localized Version" ;
        skos:prefLabel   "Singapore" .

v3-hl7Realm:CN  a        owl:Class ;
        rdfs:label       "China" ;
        rdfs:subClassOf  v3-hl7Realm:AffiliateRealms ;
        skos:definition  "Description: Realm code for use of China" ;
        skos:prefLabel   "China" .

v3-hl7Realm:RO  a        owl:Class ;
        rdfs:label       "Romania" ;
        rdfs:subClassOf  v3-hl7Realm:AffiliateRealms ;
        skos:definition  "Description: Realm code for use of Romania" ;
        skos:prefLabel   "Romania" .

v3-hl7Realm:HR  a        owl:Class ;
        rdfs:label       "Croatia" ;
        rdfs:subClassOf  v3-hl7Realm:AffiliateRealms ;
        skos:definition  "Description: Realm code for use of Croatia" ;
        skos:prefLabel   "Croatia" .

v3-hl7Realm:CH  a        owl:Class ;
        rdfs:label       "Switzerland" ;
        rdfs:subClassOf  v3-hl7Realm:AffiliateRealms ;
        skos:definition  "Description: Realm code for use of Switzerland" ;
        skos:prefLabel   "Switzerland" .

v3-hl7Realm:DK  a        owl:Class ;
        rdfs:label       "Denmark" ;
        rdfs:subClassOf  v3-hl7Realm:AffiliateRealms ;
        skos:definition  "Description: Realm code for use of Denmark" ;
        skos:prefLabel   "Denmark" .

v3-hl7Realm:C1  a        owl:Class ;
        rdfs:label       "Unclassified Realm" ;
        rdfs:subClassOf  v3-hl7Realm:BindingRealms ;
        skos:definition  "Description: Realm code for use of Unclassified Realm" ;
        skos:prefLabel   "Unclassified Realm" .

v3-hl7Realm:DE  a        owl:Class ;
        rdfs:label       "Germany" ;
        rdfs:subClassOf  v3-hl7Realm:AffiliateRealms ;
        skos:definition  "Description: Realm code for use of Germany" ;
        skos:prefLabel   "Germany" .

v3-hl7Realm:AR  a        owl:Class ;
        rdfs:label       "Argentina" ;
        rdfs:subClassOf  v3-hl7Realm:AffiliateRealms ;
        skos:definition  "Description: Realm code for use of Argentina" ;
        skos:prefLabel   "Argentina" .

v3-hl7Realm:ES  a        owl:Class ;
        rdfs:label       "Spain" ;
        rdfs:subClassOf  v3-hl7Realm:AffiliateRealms ;
        skos:definition  "Description: Realm code for use of Spain" ;
        skos:prefLabel   "Spain" .

v3-hl7Realm:IT  a        owl:Class ;
        rdfs:label       "Italy" ;
        rdfs:subClassOf  v3-hl7Realm:AffiliateRealms ;
        skos:definition  "Description: Realm code for use of Italy" ;
        skos:prefLabel   "Italy" .

v3-hl7Realm:IN  a        owl:Class ;
        rdfs:label       "India" ;
        rdfs:subClassOf  v3-hl7Realm:AffiliateRealms ;
        skos:definition  "Description: Realm code for use of India" ;
        skos:prefLabel   "India" .

v3-hl7Realm:CA  a        owl:Class ;
        rdfs:label       "Canada" ;
        rdfs:subClassOf  v3-hl7Realm:AffiliateRealms ;
        skos:definition  "Description: Realm code for use of Canada" ;
        skos:prefLabel   "Canada" .

v3-hl7Realm:GB  a        owl:Class ;
        rdfs:label       "Great Britain" ;
        rdfs:subClassOf  v3-hl7Realm:BindingRealms ;
        skos:definition  "Description: Realm code for use of Great Britain" ;
        skos:prefLabel   "Great Britain" .

v3-hl7Realm:R1  a        owl:Class ;
        rdfs:label       "Representative Realm" ;
        rdfs:subClassOf  v3-hl7Realm:BindingRealms ;
        skos:definition  "Description: Realm code for use of Representative Realm" ;
        skos:prefLabel   "Representative Realm" .

v3-hl7Realm:SE  a        owl:Class ;
        rdfs:label       "Sweden" ;
        rdfs:subClassOf  v3-hl7Realm:AffiliateRealms ;
        skos:definition  "Description: Realm code for use of Sweden" ;
        skos:prefLabel   "Sweden" .

v3-hl7Realm:CL  a        owl:Class ;
        rdfs:label       "Chile" ;
        rdfs:subClassOf  v3-hl7Realm:AffiliateRealms ;
        skos:definition  "Description: Realm code for use of Chile" ;
        skos:prefLabel   "Chile" .

v3-hl7Realm:NL  a        owl:Class ;
        rdfs:label       "The Netherlands" ;
        rdfs:subClassOf  v3-hl7Realm:AffiliateRealms ;
        skos:definition  "Description: Realm code for use of The Netherlands" ;
        skos:prefLabel   "The Netherlands" .

v3-hl7Realm:UK  a        owl:Class ;
        rdfs:label       "United Kingdom" ;
        rdfs:subClassOf  v3-hl7Realm:AffiliateRealms ;
        skos:definition  "Description: Realm code for use of United Kingdom" ;
        skos:prefLabel   "United Kingdom" .

v3-hl7Realm:BindingRealms
        a                owl:Class ;
        rdfs:label       "binding realms" ;
        skos:definition  "Description: Concepts that can be used as Binding Realms when creating Binding Statements.  These codes are permitted to appear in the InfrastructureRoot.realmCode attribute." ;
        skos:prefLabel   "binding realms" .

v3-hl7Realm:UV  a        owl:Class ;
        rdfs:label       "Universal" ;
        rdfs:subClassOf  v3-hl7Realm:AffiliateRealms ;
        skos:definition  "Description: Realm code for use of Universal realm or context, used in every instance" ;
        skos:prefLabel   "Universal" .

v3-hl7Realm:ZZ  a        owl:Class ;
        rdfs:label       "Localized Version" ;
        rdfs:subClassOf  v3-hl7Realm:NamespaceRealms ;
        skos:definition  "Description: An artifact created for local use only.  This realm namespace has no owning affiliate.  Its use is uncontrolled, i.e. anyone can create artifacts using this realm namespace.  Because of this, there is a significant likelihood of artifact identifier collisions.  Implementers are encouraged to register their artifacts under an affiliate owned and controlled namespace to avoid such collision problems where possible." ;
        skos:prefLabel   "Localized Version" .

v3-hl7Realm:JP  a        owl:Class ;
        rdfs:label       "Japan" ;
        rdfs:subClassOf  v3-hl7Realm:AffiliateRealms ;
        skos:definition  "Description: Realm code for use of Japan" ;
        skos:prefLabel   "Japan" .

v3-hl7Realm:GR  a        owl:Class ;
        rdfs:label       "Greece" ;
        rdfs:subClassOf  v3-hl7Realm:AffiliateRealms ;
        skos:definition  "Description: Realm code for use of Greece" ;
        skos:prefLabel   "Greece" .

v3-hl7Realm:FI  a        owl:Class ;
        rdfs:label       "Finland" ;
        rdfs:subClassOf  v3-hl7Realm:AffiliateRealms ;
        skos:definition  "Description: Realm code for use of Finland" ;
        skos:prefLabel   "Finland" .

v3-hl7Realm:SOA  a       owl:Class ;
        rdfs:label       "Southern Africa" ;
        rdfs:subClassOf  v3-hl7Realm:AffiliateRealms ;
        skos:definition  "Description: Realm code for use of Southern Africa" ;
        skos:prefLabel   "Southern Africa" .

v3-hl7Realm:X1  a        owl:Class ;
        rdfs:label       "Example Realm" ;
        rdfs:subClassOf  v3-hl7Realm:BindingRealms ;
        skos:definition  "Description: Realm code for use of Example Realm" ;
        skos:prefLabel   "Example Realm" .

v3-hl7Realm:TR  a        owl:Class ;
        rdfs:label       "Turkey" ;
        rdfs:subClassOf  v3-hl7Realm:AffiliateRealms ;
        skos:definition  "Description: Realm code for use of Turkey" ;
        skos:prefLabel   "Turkey" .

v3-hl7Realm:  a          owl:Ontology ;
        rdfs:comment     "  Description:\r\nCoded concepts representing Binding Realms (used for Context Binding of terminology in HL7 models)  and/or Namespace Realms (used to help ensure unique identification of HL7 artifacts). This code system is partitioned into three sections: Affiliate realms, Binding realms and Namespace realms.  All affiliate realm codes may automatically be used as both binding realms and namespace realms.  Furthermore, affiliate realms are the only realms that have authority over the creation of binding realms.  (Note that 'affiliate' includes the idea of both international affiliates and the HL7 International organization.)  All other codes must be associated with an owning affiliate realm and must appear as a specialization of _BindingRealm or _NamespaceRealm.  For affiliates whose concepts align with nations, the country codes from ISO 3166-1 2-character alpha are used for the code when possible so these codes should not be used for other realm types.  It is recommended that binding realm and namespace codes submitted by affiliates use the realm code as a prefix to avoid possible collisions with ISO codes.  However, tooling does not currently support namepace realm codes greater than 2 characters.  Open Issue:\r\nThe name of the concept property \"owningAffiliate\" should be changed to better reflect that the property value is the human readable name of the organizational entity that manages the Realm identified by the Realm Code.  Open Issue:\r\nIn spite of the inability of tooling to process codes longer than 2 characters, there is at least one realm codes ('SOA') that was added that is 3 characters in length." ;
        rdfs:label       "v3 Code System hl7Realm" ;
        owl:versionIRI   "http://hl7.org/fhir/v3/hl7Realm/2016-11-11" ;
        owl:versionInfo  "v3 Code System hl7Realm(2016-11-11)" .

v3-hl7Realm:AU  a        owl:Class ;
        rdfs:label       "Australia" ;
        rdfs:subClassOf  v3-hl7Realm:AffiliateRealms ;
        skos:definition  "Description: Realm code for use of Australia" ;
        skos:prefLabel   "Australia" .

v3-hl7Realm:KR  a        owl:Class ;
        rdfs:label       "Korea" ;
        rdfs:subClassOf  v3-hl7Realm:AffiliateRealms ;
        skos:definition  "Description: Realm code for use of Korea" ;
        skos:prefLabel   "Korea" .

v3-hl7Realm:MX  a        owl:Class ;
        rdfs:label       "Mexico" ;
        rdfs:subClassOf  v3-hl7Realm:AffiliateRealms ;
        skos:definition  "Description: Realm code for use of Mexico" ;
        skos:prefLabel   "Mexico" .

v3-hl7Realm:TW  a        owl:Class ;
        rdfs:label       "Taiwan" ;
        rdfs:subClassOf  v3-hl7Realm:AffiliateRealms ;
        skos:definition  "Description: Realm code for use of Taiwan" ;
        skos:prefLabel   "Taiwan" .

v3-hl7Realm:BR  a        owl:Class ;
        rdfs:label       "Brazil" ;
        rdfs:subClassOf  v3-hl7Realm:AffiliateRealms ;
        skos:definition  "Description: Realm code for use of Brazil" ;
        skos:prefLabel   "Brazil" .

v3-hl7Realm:NamespaceRealms
        a                owl:Class ;
        rdfs:label       "namespace realms" ;
        skos:definition  "Description: Codes that can be used in the \"realm\" portion of HL7 v3 artifact identifiers." ;
        skos:prefLabel   "namespace realms" .
