<rdf:RDF
   xmlns:rdf="http://www.w3.org/1999/02/22-rdf-syntax-ns#"
   xmlns:rdfs="http://www.w3.org/2000/01/rdf-schema#">

<rdf:Description rdf:about="http://www.w3.org/2000/10/annotation-ns#">
 <rdfs:comment>A namespace for describing annotations</rdfs:comment>
 <rdfs:comment>$Revision$ $Date$</rdfs:comment>
 <rdfs:seeAlso rdf:resource="http://www.w3.org/2000/02/Collaboration/Annotation/papers"/>
</rdf:Description>

<rdfs:Class rdf:about="http://www.w3.org/2000/10/annotation-ns#Annotation">
  <rdfs:label xml:lang="en">Annotation</rdfs:label>
  <rdfs:comment>The target type of a annotation resource.</rdfs:comment>
  <rdfs:isDefinedBy rdf:resource="http://www.w3.org/2000/10/annotation-ns#"/>
</rdfs:Class>

<rdf:Property rdf:about="http://www.w3.org/2000/10/annotation-ns#annotates">
  <rdfs:label xml:lang="en">annotates</rdfs:label>
  <rdfs:comment>Relates an Annotation to the resource to which the Annotation applies.  The inverse relation is 'hasAnnotation'</rdfs:comment>
  <rdfs:isDefinedBy rdf:resource="http://www.w3.org/2000/10/annotation-ns#"/>
</rdf:Property>

<rdf:Property rdf:about="http://www.w3.org/2000/10/annotation-ns#body">
  <rdfs:label xml:lang="en">body</rdfs:label>
  <rdfs:comment>Relates the resource representing the 'content' of an Annotation to the Annotation resource</rdfs:comment>
  <rdfs:subPropertyOf rdf:resource="http://www.w3.org/2000/10/annotation-ns#related"/>
  <rdfs:isDefinedBy rdf:resource="http://www.w3.org/2000/10/annotation-ns#"/>
</rdf:Property>

<rdf:Property rdf:about="http://www.w3.org/2000/10/annotation-ns#context">
  <rdfs:label xml:lang="en">context</rdfs:label>
  <rdfs:comment>The context within the resource named in 'annotates' to which the Annotation most directly applies.</rdfs:comment>
  <rdfs:isDefinedBy rdf:resource="http://www.w3.org/2000/10/annotation-ns#"/>
</rdf:Property>

<rdf:Property rdf:about="http://www.w3.org/2000/10/annotation-ns#author">
  <rdfs:label xml:lang="en">author</rdfs:label>
  <rdfs:comment>The name of the person or organization most responsible for creating the Annotation.</rdfs:comment>
  <rdfs:subPropertyOf rdf:resource="http://purl.org/dc/elements/1.1/creator"/>
  <rdfs:isDefinedBy rdf:resource="http://www.w3.org/2000/10/annotation-ns#"/>
</rdf:Property>

<rdf:Property rdf:about="http://www.w3.org/2000/10/annotation-ns#created">
  <rdfs:label xml:lang="en">created</rdfs:label>
  <rdfs:comment>The date and time on which the Annotation was created.  yyyy-mm-ddThh:mm:ssZ format recommended.</rdfs:comment>
  <rdfs:subPropertyOf rdf:resource="http://purl.org/dc/elements/1.1/date"/>
  <rdfs:isDefinedBy rdf:resource="http://www.w3.org/2000/10/annotation-ns#"/>
</rdf:Property>

<rdf:Property rdf:about="http://www.w3.org/2000/10/annotation-ns#modified">
  <rdfs:label xml:lang="en">modified</rdfs:label>
  <rdfs:comment>The date and time on which the Annotation was modified.  yyyy-mm-ddThh:mm:ssZ format recommended.</rdfs:comment>
  <rdfs:subPropertyOf rdf:resource="http://purl.org/dc/elements/1.1/date"/>
  <rdfs:isDefinedBy rdf:resource="http://www.w3.org/2000/10/annotation-ns#"/>
</rdf:Property>

<rdf:Property rdf:about="http://www.w3.org/2000/10/annotation-ns#related">
  <rdfs:label xml:lang="en">related</rdfs:label>
  <rdfs:comment>A relationship between an annotation and additional resources that is less specific than 'body'.  The 'related' property is expected to be
 subclassed by more specific relationships.</rdfs:comment>
  <rdfs:isDefinedBy rdf:resource="http://www.w3.org/2000/10/annotation-ns#"/>
</rdf:Property>

</rdf:RDF>
