@prefix fhir:  <http://hl7.org/fhir/> .
@prefix rdf:   <http://www.w3.org/1999/02/22-rdf-syntax-ns#> .
@prefix owl:   <http://www.w3.org/2002/07/owl#> .
@prefix xsd:   <http://www.w3.org/2001/XMLSchema#> .
@prefix v3-EntityDeterminer: <http://hl7.org/fhir/v3/EntityDeterminer/> .
@prefix skos:  <http://www.w3.org/2004/02/skos/core#> .
@prefix rdfs:  <http://www.w3.org/2000/01/rdf-schema#> .
@prefix w5:    <http://hl7.org/fhir/w5#> .

v3-EntityDeterminer:  a  owl:Ontology ;
        rdfs:comment     " EntityDeterminer in natural language grammar is the class of words that comprises articles, demonstrative pronouns, and quantifiers. In the RIM, determiner is a structural code in the Entity class to distinguish whether any given Entity object stands for some, any one, or a specific thing." ;
        rdfs:label       "v3 Code System EntityDeterminer" ;
        owl:versionIRI   "http://hl7.org/fhir/v3/EntityDeterminer/2016-11-11" ;
        owl:versionInfo  "v3 Code System EntityDeterminer(2016-11-11)" .

v3-EntityDeterminer:GROUP
        a                owl:Class ;
        rdfs:label       "specific group" ;
        rdfs:subClassOf  v3-EntityDeterminer:INSTANCE ;
        skos:definition  "A determiner that specifies that the Entity object represents a particular collection of physical things (as opposed to a universal, kind, or class of physical thing).  While the collection may resolve to having only a single individual (or even no individuals), the potential should exist for it to cover multiple individuals." ;
        skos:prefLabel   "specific group" .

v3-EntityDeterminer:KIND
        a                owl:Class ;
        rdfs:label       "described" ;
        skos:definition  "Description:A determiner that specifies that the Entity object represents a universal, kind or class of physical thing (as opposed to a particular thing)." ;
        skos:prefLabel   "described" .

v3-EntityDeterminer:INSTANCE
        a                owl:Class ;
        rdfs:label       "specific" ;
        skos:definition  "Description:A determiner that specifies that the Entity object represents a particular physical thing (as opposed to a universal, kind, or class of physical thing).\r\n\n                        \n                           Discussion: It does not matter whether an INSTANCE still exists as a whole at the point in time (or process) when we mention it, for example, a drug product lot is an INSTANCE even though it has been portioned out for retail purpose." ;
        skos:prefLabel   "specific" .

v3-EntityDeterminer:GROUPKIND
        a                owl:Class ;
        rdfs:label       "described group" ;
        rdfs:subClassOf  v3-EntityDeterminer:KIND ;
        skos:definition  "A determiner that specifies that the Entity object represents a universal, kind or class of collections physical things.  While the collection may resolve to having only a single individual (or even no individuals), the potential should exist for it to cover multiple individuals." ;
        skos:prefLabel   "described group" .

v3-EntityDeterminer:QUANTIFIED_KIND
        a                owl:Class ;
        rdfs:label       "described quantified" ;
        rdfs:subClassOf  v3-EntityDeterminer:KIND ;
        skos:definition  "The described quantified determiner indicates that the given Entity is taken as a general description of a specific amount of a thing. For example, QUANTIFIED_KIND of syringe (quantity = 3,) stands for exactly three syringes." ;
        skos:prefLabel   "described quantified" .
