@prefix v3-EntityStatus: <http://hl7.org/fhir/v3/EntityStatus/> .
@prefix fhir:  <http://hl7.org/fhir/> .
@prefix rdf:   <http://www.w3.org/1999/02/22-rdf-syntax-ns#> .
@prefix owl:   <http://www.w3.org/2002/07/owl#> .
@prefix xsd:   <http://www.w3.org/2001/XMLSchema#> .
@prefix skos:  <http://www.w3.org/2004/02/skos/core#> .
@prefix rdfs:  <http://www.w3.org/2000/01/rdf-schema#> .
@prefix w5:    <http://hl7.org/fhir/w5#> .

v3-EntityStatus:nullified
        a                owl:Class ;
        rdfs:label       "nullified" ;
        skos:definition  "The state representing the termination of an Entity record instance that was created in error." ;
        skos:prefLabel   "nullified" .

v3-EntityStatus:terminated
        a                owl:Class ;
        rdfs:label       "terminated" ;
        rdfs:subClassOf  v3-EntityStatus:normal ;
        skos:definition  "The state representing the normal termination of an Entity record." ;
        skos:prefLabel   "terminated" .

v3-EntityStatus:active
        a                owl:Class ;
        rdfs:label       "active" ;
        rdfs:subClassOf  v3-EntityStatus:normal ;
        skos:definition  "The state representing the fact that the Entity record is currently active." ;
        skos:prefLabel   "active" .

v3-EntityStatus:  a      owl:Ontology ;
        rdfs:comment     " Codes representing the defined possible states of an Entity, as defined by the Entity class state machine." ;
        rdfs:label       "v3 Code System EntityStatus" ;
        owl:versionIRI   "http://hl7.org/fhir/v3/EntityStatus/2016-11-11" ;
        owl:versionInfo  "v3 Code System EntityStatus(2016-11-11)" .

v3-EntityStatus:inactive
        a                owl:Class ;
        rdfs:label       "inactive" ;
        rdfs:subClassOf  v3-EntityStatus:normal ;
        skos:definition  "Definition: The state representing the fact that the entity is inactive." ;
        skos:prefLabel   "inactive" .

v3-EntityStatus:normal
        a                owl:Class ;
        rdfs:label       "normal" ;
        skos:definition  "The 'typical' state. Excludes \"nullified\" which represents the termination state of an Entity record instance that was created in error." ;
        skos:prefLabel   "normal" .
