@prefix fhir:  <http://hl7.org/fhir/> .
@prefix rdf:   <http://www.w3.org/1999/02/22-rdf-syntax-ns#> .
@prefix owl:   <http://www.w3.org/2002/07/owl#> .
@prefix v3-LivingArrangement: <http://hl7.org/fhir/v3/LivingArrangement/> .
@prefix xsd:   <http://www.w3.org/2001/XMLSchema#> .
@prefix skos:  <http://www.w3.org/2004/02/skos/core#> .
@prefix rdfs:  <http://www.w3.org/2000/01/rdf-schema#> .
@prefix w5:    <http://hl7.org/fhir/w5#> .

v3-LivingArrangement:SL
        a                owl:Class ;
        rdfs:label       "supported living" ;
        rdfs:subClassOf  v3-LivingArrangement:PR ;
        skos:definition  "Definition: Assisted living in a single family residence for persons with physical, behavioral, or functional health, or socio-economic challenges.  There may or may not be on-site supervision but the housing is designed to assist the client with developing independent living skills. Community based services may be provided." ;
        skos:prefLabel   "supported living" .

v3-LivingArrangement:I
        a                owl:Class ;
        rdfs:label       "Institution" ;
        skos:definition  "Institution" ;
        skos:prefLabel   "Institution" .

v3-LivingArrangement:N
        a                owl:Class ;
        rdfs:label       "Nursing Home" ;
        rdfs:subClassOf  v3-LivingArrangement:I ;
        skos:definition  "Nursing Home" ;
        skos:prefLabel   "Nursing Home" .

v3-LivingArrangement:X
        a                owl:Class ;
        rdfs:label       "Extended care facility" ;
        rdfs:subClassOf  v3-LivingArrangement:I ;
        skos:definition  "Extended care facility" ;
        skos:prefLabel   "Extended care facility" .

v3-LivingArrangement:G
        a                owl:Class ;
        rdfs:label       "Group Home" ;
        rdfs:subClassOf  v3-LivingArrangement:I ;
        skos:definition  "Group Home" ;
        skos:prefLabel   "Group Home" .

v3-LivingArrangement:T
        a                owl:Class ;
        rdfs:label       "Transient" ;
        rdfs:subClassOf  v3-LivingArrangement:HL ;
        skos:definition  "Transient" ;
        skos:prefLabel   "Transient" .

v3-LivingArrangement:H
        a                owl:Class ;
        rdfs:label       "Independent Household" ;
        rdfs:subClassOf  v3-LivingArrangement:PR ;
        skos:definition  "Independent Household" ;
        skos:prefLabel   "Independent Household" .

v3-LivingArrangement:PR
        a                owl:Class ;
        rdfs:label       "private residence" ;
        skos:definition  "Definition:  A living arrangement within a private residence for single family." ;
        skos:prefLabel   "private residence" .

v3-LivingArrangement:CS
        a                owl:Class ;
        rdfs:label       "community shelter" ;
        rdfs:subClassOf  v3-LivingArrangement:I ;
        skos:definition  "Definition: A group living arrangement specifically for the care of those in need of temporary and crisis housing assistance.  Examples include domestic violence shelters, shelters for displaced or homeless individuals, Salvation Army, Jesus House, etc.  Community based services may be provided." ;
        skos:prefLabel   "community shelter" .

v3-LivingArrangement:HL
        a                owl:Class ;
        rdfs:label       "homeless" ;
        skos:definition  "Definition: Living arrangements lacking a permanent residence." ;
        skos:prefLabel   "homeless" .

v3-LivingArrangement:
        a                owl:Ontology ;
        rdfs:comment     " A code depicting the living arrangements of a person" ;
        rdfs:label       "v3 Code System LivingArrangement" ;
        owl:versionIRI   "http://hl7.org/fhir/v3/LivingArrangement/2016-11-11" ;
        owl:versionInfo  "v3 Code System LivingArrangement(2016-11-11)" .

v3-LivingArrangement:M
        a                owl:Class ;
        rdfs:label       "Nomadic" ;
        rdfs:subClassOf  v3-LivingArrangement:HL ;
        skos:definition  "Nomadic" ;
        skos:prefLabel   "Nomadic" .

v3-LivingArrangement:R
        a                owl:Class ;
        rdfs:label       "Retirement Community" ;
        rdfs:subClassOf  v3-LivingArrangement:PR ;
        skos:definition  "Retirement Community" ;
        skos:prefLabel   "Retirement Community" .
