@prefix fhir:  <http://hl7.org/fhir/> .
@prefix rdf:   <http://www.w3.org/1999/02/22-rdf-syntax-ns#> .
@prefix owl:   <http://www.w3.org/2002/07/owl#> .
@prefix xsd:   <http://www.w3.org/2001/XMLSchema#> .
@prefix v3-EntityNameUse: <http://hl7.org/fhir/v3/EntityNameUse/> .
@prefix skos:  <http://www.w3.org/2004/02/skos/core#> .
@prefix rdfs:  <http://www.w3.org/2000/01/rdf-schema#> .
@prefix w5:    <http://hl7.org/fhir/w5#> .

v3-EntityNameUse:L  a    owl:Class ;
        rdfs:label       "Legal" ;
        skos:definition  "Known as/conventional/the one you use" ;
        skos:prefLabel   "Legal" .

v3-EntityNameUse:_NameRepresentationUse
        a                owl:Class ;
        rdfs:label       "NameRepresentationUse" ;
        skos:definition  "Identifies the different representations of a name.  The representation may affect how the name is used.  (E.g. use of Ideographic for formal communications.)" ;
        skos:prefLabel   "NameRepresentationUse" .

v3-EntityNameUse:SNDX
        a                owl:Class ;
        rdfs:label       "Soundex" ;
        rdfs:subClassOf  v3-EntityNameUse:SRCH ;
        skos:definition  "A name spelled according to the SoundEx algorithm." ;
        skos:prefLabel   "Soundex" .

v3-EntityNameUse:SYL  a  owl:Class ;
        rdfs:label       "Syllabic" ;
        rdfs:subClassOf  v3-EntityNameUse:_NameRepresentationUse ;
        skos:definition  "Syllabic transcription of name (e.g., Japanese kana, Korean hangul)" ;
        skos:prefLabel   "Syllabic" .

v3-EntityNameUse:C  a    owl:Class ;
        rdfs:label       "License" ;
        skos:definition  "As recorded on a license, record, certificate, etc. (only if different from legal name)" ;
        skos:prefLabel   "License" .

v3-EntityNameUse:R  a    owl:Class ;
        rdfs:label       "Religious" ;
        skos:definition  "e.g. Sister Mary Francis, Brother John" ;
        skos:prefLabel   "Religious" .

v3-EntityNameUse:PHON
        a                owl:Class ;
        rdfs:label       "phonetic" ;
        rdfs:subClassOf  v3-EntityNameUse:SRCH ;
        skos:definition  "A name spelled phonetically.\r\n\n                        There are a variety of phonetic spelling algorithms. This code value does not distinguish between these.Discussion:" ;
        skos:prefLabel   "phonetic" .

v3-EntityNameUse:A  a    owl:Class ;
        rdfs:label       "Artist/Stage" ;
        rdfs:subClassOf  v3-EntityNameUse:P ;
        skos:definition  "Includes writer's pseudonym, stage name, etc" ;
        skos:prefLabel   "Artist/Stage" .

v3-EntityNameUse:IDE  a  owl:Class ;
        rdfs:label       "Ideographic" ;
        rdfs:subClassOf  v3-EntityNameUse:_NameRepresentationUse ;
        skos:definition  "Ideographic representation of name (e.g., Japanese kanji, Chinese characters)" ;
        skos:prefLabel   "Ideographic" .

v3-EntityNameUse:SRCH
        a                owl:Class ;
        rdfs:label       "search" ;
        skos:definition  "A name intended for use in searching or matching." ;
        skos:prefLabel   "search" .

v3-EntityNameUse:P  a    owl:Class ;
        rdfs:label       "pseudonym" ;
        skos:definition  "A self asserted name that the person is using or has used." ;
        skos:prefLabel   "pseudonym" .

v3-EntityNameUse:ASGN
        a                owl:Class ;
        rdfs:label       "assigned" ;
        skos:definition  "A name assigned to a person. Reasons some organizations assign alternate names may include not knowing the person's name, or to maintain anonymity. Some, but not necessarily all, of the name types that people call \"alias\" may fit into this category." ;
        skos:prefLabel   "assigned" .

v3-EntityNameUse:I  a    owl:Class ;
        rdfs:label       "Indigenous/Tribal" ;
        skos:definition  "e.g. Chief Red Cloud" ;
        skos:prefLabel   "Indigenous/Tribal" .

v3-EntityNameUse:OR  a   owl:Class ;
        rdfs:label       "official registry" ;
        rdfs:subClassOf  v3-EntityNameUse:L ;
        skos:definition  "Definition:The formal name as registered in an official (government) registry, but which name might not be commonly used. Particularly used in countries with a law system based on Napoleonic law." ;
        skos:prefLabel   "official registry" .

v3-EntityNameUse:ABC  a  owl:Class ;
        rdfs:label       "Alphabetic" ;
        rdfs:subClassOf  v3-EntityNameUse:_NameRepresentationUse ;
        skos:definition  "Alphabetic transcription of name (Japanese: romaji)" ;
        skos:prefLabel   "Alphabetic" .

v3-EntityNameUse:  a     owl:Ontology ;
        rdfs:comment     "**** MISSING DEFINITIONS ****" ;
        rdfs:label       "v3 Code System EntityNameUse" ;
        owl:versionIRI   "http://hl7.org/fhir/v3/EntityNameUse/2016-11-11" ;
        owl:versionInfo  "v3 Code System EntityNameUse(2016-11-11)" .
