@prefix restful-interaction: <http://hl7.org/fhir/restful-interaction/> .
@prefix fhir:  <http://hl7.org/fhir/> .
@prefix rdf:   <http://www.w3.org/1999/02/22-rdf-syntax-ns#> .
@prefix owl:   <http://www.w3.org/2002/07/owl#> .
@prefix xsd:   <http://www.w3.org/2001/XMLSchema#> .
@prefix skos:  <http://www.w3.org/2004/02/skos/core#> .
@prefix rdfs:  <http://www.w3.org/2000/01/rdf-schema#> .
@prefix w5:    <http://hl7.org/fhir/w5#> .

restful-interaction:operation
        a                owl:Class ;
        rdfs:label       "operation" ;
        skos:definition  "Perform an operation as defined by an OperationDefinition." ;
        skos:prefLabel   "operation" .

restful-interaction:update
        a                owl:Class ;
        rdfs:label       "update" ;
        skos:definition  "Update an existing resource by its id (or create it if it is new)." ;
        skos:prefLabel   "update" .

restful-interaction:history-system
        a                owl:Class ;
        rdfs:label       "history-system" ;
        rdfs:subClassOf  restful-interaction:history ;
        skos:definition  "Retrieve the change history for all resources on a system." ;
        skos:prefLabel   "history-system" .

restful-interaction:delete
        a                owl:Class ;
        rdfs:label       "delete" ;
        skos:definition  "Delete a resource." ;
        skos:prefLabel   "delete" .

restful-interaction:history-instance
        a                owl:Class ;
        rdfs:label       "history-instance" ;
        rdfs:subClassOf  restful-interaction:history ;
        skos:definition  "Retrieve the change history for a particular resource." ;
        skos:prefLabel   "history-instance" .

restful-interaction:search
        a                owl:Class ;
        rdfs:label       "search" ;
        skos:definition  "Search a resource type or all resources based on some filter criteria." ;
        skos:prefLabel   "search" .

restful-interaction:search-type
        a                owl:Class ;
        rdfs:label       "search-type" ;
        rdfs:subClassOf  restful-interaction:search ;
        skos:definition  "Search all resources of the specified type based on some filter criteria." ;
        skos:prefLabel   "search-type" .

restful-interaction:batch
        a                owl:Class ;
        rdfs:label       "batch" ;
        skos:definition  "perform a set of a separate interactions in a single http operation" ;
        skos:prefLabel   "batch" .

restful-interaction:capabilities
        a                owl:Class ;
        rdfs:label       "capabilities" ;
        skos:definition  "Get a Capability Statement for the system." ;
        skos:prefLabel   "capabilities" .

restful-interaction:search-system
        a                owl:Class ;
        rdfs:label       "search-system" ;
        rdfs:subClassOf  restful-interaction:search ;
        skos:definition  "Search all resources based on some filter criteria." ;
        skos:prefLabel   "search-system" .

restful-interaction:patch
        a                owl:Class ;
        rdfs:label       "patch" ;
        skos:definition  "Update an existing resource by posting a set of changes to it." ;
        skos:prefLabel   "patch" .

restful-interaction:  a  owl:Ontology ;
        rdfs:comment     "The set of interactions defined by the RESTful part of the FHIR specification." ;
        rdfs:label       "FHIR Restful Interactions" ;
        owl:versionIRI   "http://hl7.org/fhir/restful-interaction/null" ;
        owl:versionInfo  "FHIR Restful Interactions(null)" .

restful-interaction:transaction
        a                owl:Class ;
        rdfs:label       "transaction" ;
        skos:definition  "Update, create or delete a set of resources as a single transaction." ;
        skos:prefLabel   "transaction" .

restful-interaction:vread
        a                owl:Class ;
        rdfs:label       "vread" ;
        skos:definition  "Read the state of a specific version of the resource." ;
        skos:prefLabel   "vread" .

restful-interaction:read
        a                owl:Class ;
        rdfs:label       "read" ;
        skos:definition  "Read the current state of the resource." ;
        skos:prefLabel   "read" .

restful-interaction:history
        a                owl:Class ;
        rdfs:label       "history" ;
        skos:definition  "Retrieve the change history for a particular resource, type of resource, or the entire system." ;
        skos:prefLabel   "history" .

restful-interaction:history-type
        a                owl:Class ;
        rdfs:label       "history-type" ;
        rdfs:subClassOf  restful-interaction:history ;
        skos:definition  "Retrieve the change history for all resources of a particular type." ;
        skos:prefLabel   "history-type" .

restful-interaction:create
        a                owl:Class ;
        rdfs:label       "create" ;
        skos:definition  "Create a new resource with a server assigned id." ;
        skos:prefLabel   "create" .
