@prefix fhir:  <http://hl7.org/fhir/> .
@prefix rdf:   <http://www.w3.org/1999/02/22-rdf-syntax-ns#> .
@prefix owl:   <http://www.w3.org/2002/07/owl#> .
@prefix xsd:   <http://www.w3.org/2001/XMLSchema#> .
@prefix skos:  <http://www.w3.org/2004/02/skos/core#> .
@prefix rdfs:  <http://www.w3.org/2000/01/rdf-schema#> .
@prefix w5:    <http://hl7.org/fhir/w5#> .
@prefix questionnaire-item-control: <http://hl7.org/fhir/questionnaire-item-control/> .

questionnaire-item-control:flyover
        a                owl:Class ;
        rdfs:label       "Fly-over" ;
        rdfs:subClassOf  questionnaire-item-control:text ;
        skos:definition  "Text is temporarily visible over top of an item if the mouse is positioned over top of the text for the containing item" ;
        skos:prefLabel   "Fly-over" .

questionnaire-item-control:prompt
        a                owl:Class ;
        rdfs:label       "Prompt" ;
        rdfs:subClassOf  questionnaire-item-control:text ;
        skos:definition  "Text is displayed immediately below or within the answer-entry area of the containing question item (typically as a guide for what to enter)" ;
        skos:prefLabel   "Prompt" .

questionnaire-item-control:list
        a                owl:Class ;
        rdfs:label       "List" ;
        rdfs:subClassOf  questionnaire-item-control:group ;
        skos:definition  "Questions within the group should be listed sequentially" ;
        skos:prefLabel   "List" .

questionnaire-item-control:group
        a                owl:Class ;
        rdfs:label       "group" ;
        skos:definition  "UI controls relevant to organizing groups of questions" ;
        skos:prefLabel   "group" .

questionnaire-item-control:autocomplete
        a                owl:Class ;
        rdfs:label       "Auto-complete" ;
        rdfs:subClassOf  questionnaire-item-control:question ;
        skos:definition  "A control which provides a list of potential matches based on text entered into a control.  Used for large choice sets where text-matching is an appropriate discovery mechanism." ;
        skos:prefLabel   "Auto-complete" .

questionnaire-item-control:unit
        a                owl:Class ;
        rdfs:label       "Unit" ;
        rdfs:subClassOf  questionnaire-item-control:text ;
        skos:definition  "Text is displayed adjacent (horizontally or vertically) to the answer space for the parent question, typically to indicate a unit of measure" ;
        skos:prefLabel   "Unit" .

questionnaire-item-control:help
        a                owl:Class ;
        rdfs:label       "Help-Button" ;
        rdfs:subClassOf  questionnaire-item-control:text ;
        skos:definition  "Text is displayed in a dialog box or similar control if invoked by pushing a button or some other UI-appropriate action to request 'help' for a question, group or the questionnaire as a whole (depending what the text is nested within)" ;
        skos:prefLabel   "Help-Button" .

questionnaire-item-control:text
        a                owl:Class ;
        rdfs:label       "text" ;
        skos:definition  "UI controls relevant to rendering questionnaire text items" ;
        skos:prefLabel   "text" .

questionnaire-item-control:check-box
        a                owl:Class ;
        rdfs:label       "Check-box" ;
        rdfs:subClassOf  questionnaire-item-control:question ;
        skos:definition  "A control where choices are listed with a box beside them.  The box can be toggled to select or de-select a given choice.  Multiple selections may be possible." ;
        skos:prefLabel   "Check-box" .

questionnaire-item-control:lower
        a                owl:Class ;
        rdfs:label       "Lower-bound" ;
        rdfs:subClassOf  questionnaire-item-control:text ;
        skos:definition  "Text is displayed to the left of the set of answer choices or a scaling control for the parent question item to indicate the meaning of the 'lower' bound.  E.g. 'Strongly disagree'" ;
        skos:prefLabel   "Lower-bound" .

questionnaire-item-control:lookup
        a                owl:Class ;
        rdfs:label       "Lookup" ;
        rdfs:subClassOf  questionnaire-item-control:question ;
        skos:definition  "A control where editing an item spawns a separate dialog box or screen permitting a user to navigate, filter or otherwise discover an appropriate match.  Useful for large choice sets where text matching is not an appropriate discovery mechanism.  Such screens must generally be tuned for the specific choice list structure." ;
        skos:prefLabel   "Lookup" .

questionnaire-item-control:drop-down
        a                owl:Class ;
        rdfs:label       "Drop down" ;
        rdfs:subClassOf  questionnaire-item-control:question ;
        skos:definition  "A control where an item (or multiple items) can be selected from a list that is only displayed when the user is editing the field." ;
        skos:prefLabel   "Drop down" .

questionnaire-item-control:question
        a                owl:Class ;
        rdfs:label       "question" ;
        skos:definition  "UI controls relevant to capturing question data" ;
        skos:prefLabel   "question" .

questionnaire-item-control:inline
        a                owl:Class ;
        rdfs:label       "In-line" ;
        rdfs:subClassOf  questionnaire-item-control:text ;
        skos:definition  "Text is displayed as a paragraph in a sequential position between sibling items (default behavior)" ;
        skos:prefLabel   "In-line" .

questionnaire-item-control:slider
        a                owl:Class ;
        rdfs:label       "Slider" ;
        rdfs:subClassOf  questionnaire-item-control:question ;
        skos:definition  "A control where an axis is displayed between the high and low values and the control can be visually manipulated to select a value anywhere on the axis." ;
        skos:prefLabel   "Slider" .

questionnaire-item-control:text-box
        a                owl:Class ;
        rdfs:label       "Text Box" ;
        rdfs:subClassOf  questionnaire-item-control:question ;
        skos:definition  "A control where a user can type in their answer freely." ;
        skos:prefLabel   "Text Box" .

questionnaire-item-control:spinner
        a                owl:Class ;
        rdfs:label       "Spinner" ;
        rdfs:subClassOf  questionnaire-item-control:question ;
        skos:definition  "A control where a list of numeric or other ordered values can be scrolled through via arrows." ;
        skos:prefLabel   "Spinner" .

questionnaire-item-control:footer
        a                owl:Class ;
        rdfs:label       "Footer" ;
        rdfs:subClassOf  questionnaire-item-control:group ;
        skos:definition  "The group is to be continuously visible at the bottom of the questionnaire" ;
        skos:prefLabel   "Footer" .

questionnaire-item-control:header
        a                owl:Class ;
        rdfs:label       "Header" ;
        rdfs:subClassOf  questionnaire-item-control:group ;
        skos:definition  "The group is to be continuously visible at the top of the questionnaire" ;
        skos:prefLabel   "Header" .

questionnaire-item-control:table
        a                owl:Class ;
        rdfs:label       "Table" ;
        rdfs:subClassOf  questionnaire-item-control:group ;
        skos:definition  "Questions within the group are rows in the table with possible answers as columns" ;
        skos:prefLabel   "Table" .

questionnaire-item-control:
        a                owl:Ontology ;
        rdfs:comment     "Starter set of user interface control/display mechanisms that might be used when rendering an item in a questionnaire." ;
        rdfs:label       "Questionnaire Item UI Control Codes" ;
        owl:versionIRI   "http://hl7.org/fhir/questionnaire-item-control/3.1.0" ;
        owl:versionInfo  "Questionnaire Item UI Control Codes(3.1.0)" .

questionnaire-item-control:radio-button
        a                owl:Class ;
        rdfs:label       "Radio Button" ;
        rdfs:subClassOf  questionnaire-item-control:question ;
        skos:definition  "A control where choices are listed with a button beside them.  The button can be toggled to select or de-select a given choice.  Selecting one item deselects all others." ;
        skos:prefLabel   "Radio Button" .

questionnaire-item-control:upper
        a                owl:Class ;
        rdfs:label       "Upper-bound" ;
        rdfs:subClassOf  questionnaire-item-control:text ;
        skos:definition  "Text is displayed to the right of the set of answer choices or a scaling control for the parent question item to indicate the meaning of the 'upper' bound.  E.g. 'Strongly agree'" ;
        skos:prefLabel   "Upper-bound" .
