# baseURI: https://www.w3.org/2006/time/rel
# imports: http://purl.org/dc/elements/1.1/
# imports: http://www.w3.org/2006/time
# prefix: rel

@prefix dct: <http://purl.org/dc/terms/> .
@prefix owl: <http://www.w3.org/2002/07/owl#> .
@prefix rdf: <http://www.w3.org/1999/02/22-rdf-syntax-ns#> .
@prefix rdfs: <http://www.w3.org/2000/01/rdf-schema#> .
@prefix rel: <https://www.w3.org/2006/time/rel#> .
@prefix skos: <http://www.w3.org/2004/02/skos/core#> .
@prefix time: <http://www.w3.org/2006/time#> .
@prefix xsd: <http://www.w3.org/2001/XMLSchema#> .

time:after
  rdfs:subPropertyOf time:disjoint ;
.
time:before
  rdfs:subPropertyOf time:disjoint ;
.
time:disjoint
  a owl:ObjectProperty ;
  rdfs:comment "If a temporal entity T1 is disjoint with another temporal entity T2, then the beginning of T1 is after the end of T2, or the end of T1 is before the beginning of T2, i.e. the two entities do not overlap or coincide in any way, but their ordering relationship is not known."@en ;
  rdfs:domain time:TemporalEntity ;
  rdfs:label "disjoint time entity" ;
  rdfs:range time:TemporalEntity ;
  owl:propertyDisjointWith time:notDisjoint ;
  skos:example """
ex:LunchTime time:disjoint ex:NapTime .
""" ;
.
time:equals
  a owl:ObjectProperty ;
  rdfs:comment "If a temporal entity T1 equals another temporal entity T2, then the beginning of T1 is coincident with the beginning of T2, and the end of T1 is coincident with the end of T2, and the beginning of T1 may be coincident with the end of T1."@en ;
  rdfs:domain time:TemporalEntity ;
  rdfs:label "equal time entity" ;
  rdfs:range time:TemporalEntity ;
  rdfs:subPropertyOf time:notDisjoint ;
  skos:example """
ex:JackWeddingDay time:equals ex:AbbyBirthday2020 .
""" ;
.
time:hasInside
  a owl:ObjectProperty ;
  rdfs:comment "If a temporal entity T1 hasInside it another temporal entity T2, then the beginning of T1 is coincident with or before the beginning of T2, and the end of T1 is concident with or after the end of T2, except that end of T1 may not be coincident with the end of T2 if the beginning of T1 is coincident with the beginning of T2."@en ;
  rdfs:domain time:TemporalEntity ;
  rdfs:label "has time entity inside" ;
  rdfs:range time:TemporalEntity ;
  rdfs:subPropertyOf time:notDisjoint ;
  owl:propertyDisjointWith time:equals ;
  skos:example """
ex:Class time:hasInside ex:Quiz .
""" ;
.
time:inside
  rdfs:subPropertyOf time:hasInside ;
.
time:intervalContains
  rdfs:subPropertyOf time:hasInside ;
.
time:intervalDisjoint
  rdfs:subPropertyOf time:disjoint ;
.
time:intervalEquals
  rdfs:subPropertyOf time:equals ;
.
time:intervalFinishedBy
  rdfs:subPropertyOf time:hasInside ;
.
time:intervalIn
  rdfs:subPropertyOf time:notDisjoint ;
.
time:intervalMeets
  rdfs:subPropertyOf time:notDisjoint ;
.
time:intervalMetBy
  rdfs:subPropertyOf time:notDisjoint ;
.
time:intervalOverlappedBy
  rdfs:subPropertyOf time:notDisjoint ;
.
time:intervalOverlaps
  rdfs:subPropertyOf time:notDisjoint ;
.
time:intervalStartedBy
  rdfs:subPropertyOf time:hasInside ;
.
time:notDisjoint
  a owl:ObjectProperty ;
  rdfs:comment "If a temporal entity T1 is notDisjoint with another temporal entity T2, then the the two entities not overlap or coincide in some way, but their ordering relationship is not known. This relation is the complement of disjoint and the union of equals, hasInside, in, meets, metBy, overlaps, overlappedBy."@en ;
  rdfs:domain time:TemporalEntity ;
  rdfs:label "not disjoint with time entity" ;
  rdfs:range time:TemporalEntity ;
  owl:propertyDisjointWith time:disjoint ;
.
<https://www.w3.org/2006/time/rel>
  a owl:Ontology ;
  dct:created "2019-07-15"^^xsd:date ;
  dct:creator <https://orcid.org/0000-0002-3884-3420> ;
  dct:license <https://creativecommons.org/share-your-work/public-domain/cc0/> ;
  dct:modified "2020-01-16"^^xsd:date ;
  dct:title "An extension of OWL-Time for temporal entity relations" ;
  rdfs:label "Temporal entity relations" ;
  rdfs:comment """This document describes some extensions to OWL-Time to represent relationships between temporal entities that were difficult to express using existing relationships. 
  New elements are specified in the original OWL-Time namespace. 
  These are described in https://w3c.github.io/sdw/time-entity-relations/
  Their status is non-normative, and OWL-Time applications are not required to recognize or support them. """ ;
  owl:imports <http://purl.org/dc/elements/1.1/> ;
  owl:imports <http://www.w3.org/2006/time> ;
.
