@prefix v3-QueryParameterValue: <http://hl7.org/fhir/v3/QueryParameterValue/> .
@prefix fhir:  <http://hl7.org/fhir/> .
@prefix rdf:   <http://www.w3.org/1999/02/22-rdf-syntax-ns#> .
@prefix owl:   <http://www.w3.org/2002/07/owl#> .
@prefix xsd:   <http://www.w3.org/2001/XMLSchema#> .
@prefix skos:  <http://www.w3.org/2004/02/skos/core#> .
@prefix rdfs:  <http://www.w3.org/2000/01/rdf-schema#> .
@prefix w5:    <http://hl7.org/fhir/w5#> .

v3-QueryParameterValue:_DispenseQueryFilterCode
        a                owl:Class ;
        rdfs:label       "dispense query filter code" ;
        skos:definition  "Description:Filter codes used to manage volume of dispenses returned by  a parameter-based queries." ;
        skos:prefLabel   "dispense query filter code" .

v3-QueryParameterValue:_PrescriptionDispenseFilterCode
        a                owl:Class ;
        rdfs:label       "Prescription Dispense Filter Code" ;
        skos:definition  "A \"helper\" vocabulary used to construct complex query filters based on how and whether a prescription has been dispensed." ;
        skos:prefLabel   "Prescription Dispense Filter Code" .

v3-QueryParameterValue:NODISP
        a                owl:Class ;
        rdfs:label       "no dispense" ;
        rdfs:subClassOf  v3-QueryParameterValue:_DispenseQueryFilterCode ;
        skos:definition  "Description:Returns no dispense for a prescription." ;
        skos:prefLabel   "no dispense" .

v3-QueryParameterValue:_QueryParameterValue
        a                owl:Class ;
        rdfs:label       "QueryParameterValue" ;
        skos:definition  "Description:Indicates how result sets should be filtered based on whether they have associated issues." ;
        skos:prefLabel   "QueryParameterValue" .

v3-QueryParameterValue:ISSFA
        a                owl:Class ;
        rdfs:label       "all" ;
        rdfs:subClassOf  v3-QueryParameterValue:_QueryParameterValue ;
        skos:definition  "Description:Result set should not be filtered based on the presence of issues." ;
        skos:prefLabel   "all" .

v3-QueryParameterValue:ISSFU
        a                owl:Class ;
        rdfs:label       "with unmanaged issues" ;
        rdfs:subClassOf  v3-QueryParameterValue:_QueryParameterValue ;
        skos:definition  "Description:Result set should be filtered to only include records with associated unmanaged issues." ;
        skos:prefLabel   "with unmanaged issues" .

v3-QueryParameterValue:ISSFI
        a                owl:Class ;
        rdfs:label       "with issues" ;
        rdfs:subClassOf  v3-QueryParameterValue:_QueryParameterValue ;
        skos:definition  "Description:Result set should be filtered to only include records with associated issues." ;
        skos:prefLabel   "with issues" .

v3-QueryParameterValue:C
        a                owl:Class ;
        rdfs:label       "Completely dispensed" ;
        rdfs:subClassOf  v3-QueryParameterValue:_PrescriptionDispenseFilterCode ;
        skos:definition  "Filter to only include SubstanceAdministration orders which have no remaining quantity authorized to be dispensed." ;
        skos:prefLabel   "Completely dispensed" .

v3-QueryParameterValue:LASTDISP
        a                owl:Class ;
        rdfs:label       "last dispense" ;
        rdfs:subClassOf  v3-QueryParameterValue:_DispenseQueryFilterCode ;
        skos:definition  "Description:Returns the most recent dispense for a prescription." ;
        skos:prefLabel   "last dispense" .

v3-QueryParameterValue:R
        a                owl:Class ;
        rdfs:label       "Dispensed with remaining fills" ;
        rdfs:subClassOf  v3-QueryParameterValue:_PrescriptionDispenseFilterCode ;
        skos:definition  "Filter to only include SubstanceAdministration orders which have had at least one fulfilling supply event, but which still have outstanding quantity remaining to be authorized." ;
        skos:prefLabel   "Dispensed with remaining fills" .

v3-QueryParameterValue:ONR
        a                owl:Class ;
        rdfs:label       "orders without results" ;
        rdfs:subClassOf  v3-QueryParameterValue:_OrderFilterCode ;
        skos:definition  "Return only those orders that do not have results." ;
        skos:prefLabel   "orders without results" .

v3-QueryParameterValue:OWR
        a                owl:Class ;
        rdfs:label       "orders with results" ;
        rdfs:subClassOf  v3-QueryParameterValue:_OrderFilterCode ;
        skos:definition  "Return only those orders that have results." ;
        skos:prefLabel   "orders with results" .

v3-QueryParameterValue:AO
        a                owl:Class ;
        rdfs:label       "all orders" ;
        rdfs:subClassOf  v3-QueryParameterValue:_OrderFilterCode ;
        skos:definition  "Return all orders." ;
        skos:prefLabel   "all orders" .

v3-QueryParameterValue:_OrderFilterCode
        a                owl:Class ;
        rdfs:label       "_OrderFilterCode" ;
        skos:definition  "Filter codes used to manage types of orders being returned by a parameter-based query." ;
        skos:prefLabel   "_OrderFilterCode" .

v3-QueryParameterValue:ALLDISP
        a                owl:Class ;
        rdfs:label       "all dispenses" ;
        rdfs:subClassOf  v3-QueryParameterValue:_DispenseQueryFilterCode ;
        skos:definition  "Description:Returns all dispenses to date for a prescription." ;
        skos:prefLabel   "all dispenses" .

v3-QueryParameterValue:
        a                owl:Ontology ;
        rdfs:comment     " The domain of coded values used as parameters within QueryByParameter queries." ;
        rdfs:label       "v3 Code System QueryParameterValue" ;
        owl:versionIRI   "http://hl7.org/fhir/v3/QueryParameterValue/2016-11-11" ;
        owl:versionInfo  "v3 Code System QueryParameterValue(2016-11-11)" .

v3-QueryParameterValue:N
        a                owl:Class ;
        rdfs:label       "Never Dispensed" ;
        rdfs:subClassOf  v3-QueryParameterValue:_PrescriptionDispenseFilterCode ;
        skos:definition  "Filter to only include SubstanceAdministration orders which have no fulfilling supply events performed." ;
        skos:prefLabel   "Never Dispensed" .
