@prefix v3-EntityNameUseR2: <http://hl7.org/fhir/v3/EntityNameUseR2/> .
@prefix fhir:  <http://hl7.org/fhir/> .
@prefix rdf:   <http://www.w3.org/1999/02/22-rdf-syntax-ns#> .
@prefix owl:   <http://www.w3.org/2002/07/owl#> .
@prefix xsd:   <http://www.w3.org/2001/XMLSchema#> .
@prefix skos:  <http://www.w3.org/2004/02/skos/core#> .
@prefix rdfs:  <http://www.w3.org/2000/01/rdf-schema#> .
@prefix w5:    <http://hl7.org/fhir/w5#> .

v3-EntityNameUseR2:A  a  owl:Class ;
        rdfs:label       "business name" ;
        rdfs:subClassOf  v3-EntityNameUseR2:Assumed ;
        skos:definition  "Description:A name used in a Professional or Business context .  Examples: Continuing to use a maiden name in a professional context, or using a stage performing name (some of these names are also pseudonyms)" ;
        skos:prefLabel   "business name" .

v3-EntityNameUseR2:M  a  owl:Class ;
        rdfs:label       "maiden name" ;
        skos:definition  "Description:A name used prior to marriage.Note that marriage naming customs vary greatly around the world.  This name use is for use by applications that collect and store maiden names.  Though the concept of maiden name is often gender specific, the use of this term is not gender specific.  The use of this term does not imply any particular history for a person's name, nor should the maiden name be determined algorithmically" ;
        skos:prefLabel   "maiden name" .

v3-EntityNameUseR2:IDE
        a                owl:Class ;
        rdfs:label       "ideographic" ;
        rdfs:subClassOf  v3-EntityNameUseR2:NameRepresentationUse ;
        skos:definition  "Description:Ideographic representation of name (e.g., Japanese kanji, Chinese characters)" ;
        skos:prefLabel   "ideographic" .

v3-EntityNameUseR2:R  a  owl:Class ;
        rdfs:label       "religious" ;
        rdfs:subClassOf  v3-EntityNameUseR2:Assumed ;
        skos:definition  "Description:A name assumed as part of a religious vocation .  e.g .  Sister Mary Francis, Brother John" ;
        skos:prefLabel   "religious" .

v3-EntityNameUseR2:SRCH
        a                owl:Class ;
        rdfs:label       "search" ;
        skos:definition  "Description:A name intended for use in searching or matching.  This is used when the name is incomplete and contains enough details for search matching, but not enough for other uses." ;
        skos:prefLabel   "search" .

v3-EntityNameUseR2:NameRepresentationUse
        a                owl:Class ;
        rdfs:label       "NameRepresentationUse" ;
        skos:definition  "Description:Identifies the different representations of a name .  The representation may affect how the name is used .  (E.g .  use of Ideographic for formal communications.)" ;
        skos:prefLabel   "NameRepresentationUse" .

v3-EntityNameUseR2:  a   owl:Ontology ;
        rdfs:comment     "  Description:\r\nA set of codes advising a system or user which name in a set of names to select for a given purpose." ;
        rdfs:label       "v3 Code System EntityNameUseR2" ;
        owl:versionIRI   "http://hl7.org/fhir/v3/EntityNameUseR2/2016-11-11" ;
        owl:versionInfo  "v3 Code System EntityNameUseR2(2016-11-11)" .

v3-EntityNameUseR2:PHON
        a                owl:Class ;
        rdfs:label       "phonetic" ;
        skos:definition  "Description:The name as understood by the data enterer, i.e. a close approximation of a phonetic spelling of the name, not based on a phonetic algorithm." ;
        skos:prefLabel   "phonetic" .

v3-EntityNameUseR2:SYL
        a                owl:Class ;
        rdfs:label       "syllabic" ;
        rdfs:subClassOf  v3-EntityNameUseR2:NameRepresentationUse ;
        skos:definition  "Description:Syllabic transcription of name (e.g., Japanese kana, Korean hangul)" ;
        skos:prefLabel   "syllabic" .

v3-EntityNameUseR2:P  a  owl:Class ;
        rdfs:label       "Other/Pseudonym/Alias" ;
        rdfs:subClassOf  v3-EntityNameUseR2:Assumed ;
        skos:definition  "Description:A non-official name by which the person is sometimes known.  (This may also be used to record informal names such as a nickname)" ;
        skos:prefLabel   "Other/Pseudonym/Alias" .

v3-EntityNameUseR2:OLD
        a                owl:Class ;
        rdfs:label       "no longer in use" ;
        skos:definition  "Description:This name is no longer in use (note: Names may also carry valid time ranges .  This code is used to cover the situations where it is known that the name is no longer valid, but no particular time range for its use is known)" ;
        skos:prefLabel   "no longer in use" .

v3-EntityNameUseR2:DN
        a                owl:Class ;
        rdfs:label       "do not use" ;
        rdfs:subClassOf  v3-EntityNameUseR2:OLD ;
        skos:definition  "Description:This name should no longer be used when interacting with the person (i.e .  in addition to no longer being used, the name should not be even mentioned when interacting with the person)Note: applications are not required to compare names labeled \"Do Not Use\" and other names in order to eliminate name parts that are common between the other name and a name labeled \"Do Not Use\"." ;
        skos:prefLabel   "do not use" .

v3-EntityNameUseR2:ANON
        a                owl:Class ;
        rdfs:label       "Anonymous" ;
        rdfs:subClassOf  v3-EntityNameUseR2:Assumed ;
        skos:definition  "Description:Anonymous assigned name (used to protect a persons identity for privacy reasons)" ;
        skos:prefLabel   "Anonymous" .

v3-EntityNameUseR2:C  a  owl:Class ;
        rdfs:label       "customary" ;
        skos:definition  "Description:Known as/conventional/the one you normally use" ;
        skos:prefLabel   "customary" .

v3-EntityNameUseR2:I  a  owl:Class ;
        rdfs:label       "Indigenous/Tribal" ;
        rdfs:subClassOf  v3-EntityNameUseR2:Assumed ;
        skos:definition  "Description:e.g .  Chief Red Cloud" ;
        skos:prefLabel   "Indigenous/Tribal" .

v3-EntityNameUseR2:ABC
        a                owl:Class ;
        rdfs:label       "alphabetic" ;
        rdfs:subClassOf  v3-EntityNameUseR2:NameRepresentationUse ;
        skos:definition  "Description:Alphabetic transcription of name in latin alphabet (Japanese: romaji)" ;
        skos:prefLabel   "alphabetic" .

v3-EntityNameUseR2:T  a  owl:Class ;
        rdfs:label       "temporary" ;
        skos:definition  "Description:A temporary name.  Note that a name valid time can provide more detailed information.  This may also be used for temporary names assigned at birth or in emergency situations." ;
        skos:prefLabel   "temporary" .

v3-EntityNameUseR2:OR
        a                owl:Class ;
        rdfs:label       "official registry name" ;
        skos:definition  "Description:The formal name as registered in an official (government) registry, but which name might not be commonly used .  May correspond to the concept of legal name" ;
        skos:prefLabel   "official registry name" .

v3-EntityNameUseR2:Assumed
        a                owl:Class ;
        rdfs:label       "Assumed" ;
        skos:definition  "Description:A name that a person has assumed or has been assumed to them." ;
        skos:prefLabel   "Assumed" .
