@prefix v3-ManagedParticipationStatus: <http://hl7.org/fhir/v3/ManagedParticipationStatus/> .
@prefix fhir:  <http://hl7.org/fhir/> .
@prefix rdf:   <http://www.w3.org/1999/02/22-rdf-syntax-ns#> .
@prefix owl:   <http://www.w3.org/2002/07/owl#> .
@prefix xsd:   <http://www.w3.org/2001/XMLSchema#> .
@prefix skos:  <http://www.w3.org/2004/02/skos/core#> .
@prefix rdfs:  <http://www.w3.org/2000/01/rdf-schema#> .
@prefix w5:    <http://hl7.org/fhir/w5#> .

v3-ManagedParticipationStatus:cancelled
        a                owl:Class ;
        rdfs:label       "cancelled" ;
        rdfs:subClassOf  v3-ManagedParticipationStatus:normal ;
        skos:definition  "The terminal state resulting from cancellation of the Participation prior to activation." ;
        skos:prefLabel   "cancelled" .

v3-ManagedParticipationStatus:pending
        a                owl:Class ;
        rdfs:label       "pending" ;
        rdfs:subClassOf  v3-ManagedParticipationStatus:normal ;
        skos:definition  "The state representing that fact that the Participation has not yet become active." ;
        skos:prefLabel   "pending" .

v3-ManagedParticipationStatus:
        a                owl:Ontology ;
        rdfs:comment     " Codes representing the defined possible states of a Managed Participation, as defined by the Managed Participation class state machine." ;
        rdfs:label       "v3 Code System ManagedParticipationStatus" ;
        owl:versionIRI   "http://hl7.org/fhir/v3/ManagedParticipationStatus/2016-11-11" ;
        owl:versionInfo  "v3 Code System ManagedParticipationStatus(2016-11-11)" .

v3-ManagedParticipationStatus:completed
        a                owl:Class ;
        rdfs:label       "completed" ;
        rdfs:subClassOf  v3-ManagedParticipationStatus:normal ;
        skos:definition  "The terminal state representing the successful completion of the Participation." ;
        skos:prefLabel   "completed" .

v3-ManagedParticipationStatus:normal
        a                owl:Class ;
        rdfs:label       "normal" ;
        skos:definition  "The 'typical' state. Excludes \"nullified\" which represents the termination state of a participation instance that was created in error." ;
        skos:prefLabel   "normal" .

v3-ManagedParticipationStatus:active
        a                owl:Class ;
        rdfs:label       "active" ;
        rdfs:subClassOf  v3-ManagedParticipationStatus:normal ;
        skos:definition  "The state representing the fact that the Participation is in progress." ;
        skos:prefLabel   "active" .

v3-ManagedParticipationStatus:nullified
        a                owl:Class ;
        rdfs:label       "nullified" ;
        skos:definition  "The state representing the termination of a Participation instance that was created in error." ;
        skos:prefLabel   "nullified" .
