@prefix fhir:  <http://hl7.org/fhir/> .
@prefix rdf:   <http://www.w3.org/1999/02/22-rdf-syntax-ns#> .
@prefix owl:   <http://www.w3.org/2002/07/owl#> .
@prefix xsd:   <http://www.w3.org/2001/XMLSchema#> .
@prefix skos:  <http://www.w3.org/2004/02/skos/core#> .
@prefix rdfs:  <http://www.w3.org/2000/01/rdf-schema#> .
@prefix v3-AcknowledgementDetailCode: <http://hl7.org/fhir/v3/AcknowledgementDetailCode/> .
@prefix w5:    <http://hl7.org/fhir/w5#> .

v3-AcknowledgementDetailCode:NS200
        a                owl:Class ;
        rdfs:label       "Unsupported interaction" ;
        rdfs:subClassOf  v3-AcknowledgementDetailCode:_AcknowledgementDetailNotSupportedCode ;
        skos:definition  "The interaction (or: this version of the interaction) is not supported." ;
        skos:prefLabel   "Unsupported interaction" .

v3-AcknowledgementDetailCode:SYN112
        a                owl:Class ;
        rdfs:label       "Number of attribute repetitions exceeds limit" ;
        rdfs:subClassOf  v3-AcknowledgementDetailCode:SYN108 ;
        skos:definition  "The number of repetitions of an attribute exceeds the limits of the standard or of one of the conformance profiles identified in the message." ;
        skos:prefLabel   "Number of attribute repetitions exceeds limit" .

v3-AcknowledgementDetailCode:RTWDEST
        a                owl:Class ;
        rdfs:label       "Message routing warning, destination unreachable." ;
        skos:definition  "Warning: The destination of this message is known to the receiving application. Messages have been successfully routed to that destination in the past. The link to the destination application or an intermediate application is (temporarily) unavailable. The receiving application will forward the message as soon as the destination can be reached again." ;
        skos:prefLabel   "Message routing warning, destination unreachable." .

v3-AcknowledgementDetailCode:SYN102
        a                owl:Class ;
        rdfs:label       "Data type error" ;
        rdfs:subClassOf  v3-AcknowledgementDetailCode:SYN ;
        skos:definition  "The attribute contained data of the wrong data type, e.g. a numeric attribute contained \"FOO\"." ;
        skos:prefLabel   "Data type error" .

v3-AcknowledgementDetailCode:SYN108
        a                owl:Class ;
        rdfs:label       "Number of repetitions exceeds limit" ;
        rdfs:subClassOf  v3-AcknowledgementDetailCode:SYN ;
        skos:definition  "Description: The number of repetitions of a (group of) association(s) or attribute(s) exceeds the limits of the standard or of one of the conformance profiles or templates identified in the message." ;
        skos:prefLabel   "Number of repetitions exceeds limit" .

v3-AcknowledgementDetailCode:RTEDEST
        a                owl:Class ;
        rdfs:label       "Message routing error, destination unreachable." ;
        skos:definition  "Error: The destination of this message is known to the receiving application. Messages have been successfully routed to that destination in the past. The link to the destination application or an intermediate application is unavailable." ;
        skos:prefLabel   "Message routing error, destination unreachable." .

v3-AcknowledgementDetailCode:SYN111
        a                owl:Class ;
        rdfs:label       "Value does not match fixed value" ;
        rdfs:subClassOf  v3-AcknowledgementDetailCode:SYN ;
        skos:definition  "Description: The value of an attribute or property differs from the fixed value asserted in the standard or one of the conformance profiles or templates declared in the message." ;
        skos:prefLabel   "Value does not match fixed value" .

v3-AcknowledgementDetailCode:
        a                owl:Ontology ;
        rdfs:comment     "  OpenIssue:\r\nMissing description." ;
        rdfs:label       "v3 Code System AcknowledgementDetailCode" ;
        owl:versionIRI   "http://hl7.org/fhir/v3/AcknowledgementDetailCode/2016-11-11" ;
        owl:versionInfo  "v3 Code System AcknowledgementDetailCode(2016-11-11)" .

v3-AcknowledgementDetailCode:NS261
        a                owl:Class ;
        rdfs:label       "Unrecognized attentionline" ;
        rdfs:subClassOf  v3-AcknowledgementDetailCode:_AcknowledgementDetailNotSupportedCode ;
        skos:definition  "The receiver requires information in the attentionLine classes for routing purposes." ;
        skos:prefLabel   "Unrecognized attentionline" .

v3-AcknowledgementDetailCode:SYN101
        a                owl:Class ;
        rdfs:label       "Required attribute missing" ;
        rdfs:subClassOf  v3-AcknowledgementDetailCode:SYN105 ;
        skos:definition  "A required attribute is missing in a class." ;
        skos:prefLabel   "Required attribute missing" .

v3-AcknowledgementDetailCode:SYN107
        a                owl:Class ;
        rdfs:label       "Deprecated code" ;
        rdfs:subClassOf  v3-AcknowledgementDetailCode:SYN106 ;
        skos:definition  "Description: A coded attribute is referencing a code that has been deprecated by the owning code system." ;
        skos:prefLabel   "Deprecated code" .

v3-AcknowledgementDetailCode:SYN110
        a                owl:Class ;
        rdfs:label       "Number of association repetitions exceeds limit" ;
        rdfs:subClassOf  v3-AcknowledgementDetailCode:SYN108 ;
        skos:definition  "The number of repetitions of a (group of) association(s) exceeds the limits of the standard or of one of the conformance profiles identified in the message." ;
        skos:prefLabel   "Number of association repetitions exceeds limit" .

v3-AcknowledgementDetailCode:_AcknowledgementDetailNotSupportedCode
        a                owl:Class ;
        rdfs:label       "AcknowledgementDetailNotSupportedCode" ;
        skos:definition  "Refelects rejections because elements of the communication are not supported in the current context." ;
        skos:prefLabel   "AcknowledgementDetailNotSupportedCode" .

v3-AcknowledgementDetailCode:NS260
        a                owl:Class ;
        rdfs:label       "Unknown sender" ;
        rdfs:subClassOf  v3-AcknowledgementDetailCode:_AcknowledgementDetailNotSupportedCode ;
        skos:definition  "The Device.id of the sender is unknown." ;
        skos:prefLabel   "Unknown sender" .

v3-AcknowledgementDetailCode:NOSTORE
        a                owl:Class ;
        rdfs:label       "No storage space for message." ;
        skos:definition  "Rejection: The message can't be stored by the receiver due to an unspecified internal application issue. The message was neither processed nor stored by the receiving application." ;
        skos:prefLabel   "No storage space for message." .

v3-AcknowledgementDetailCode:SYN100
        a                owl:Class ;
        rdfs:label       "Required association missing" ;
        rdfs:subClassOf  v3-AcknowledgementDetailCode:SYN105 ;
        skos:definition  "Required association missing in message; or the sequence of the classes is different than required by the standard or one of the conformance profiles identified in the message." ;
        skos:prefLabel   "Required association missing" .

v3-AcknowledgementDetailCode:SYN106
        a                owl:Class ;
        rdfs:label       "Terminology error" ;
        rdfs:subClassOf  v3-AcknowledgementDetailCode:SYN ;
        skos:definition  "Description: A coded attribute or datatype property violates one of the terminology constraints specified in the standard or one of the conformance profiles or templates declared by the instance." ;
        skos:prefLabel   "Terminology error" .

v3-AcknowledgementDetailCode:NS250
        a                owl:Class ;
        rdfs:label       "Unsupported processing Mode" ;
        rdfs:subClassOf  v3-AcknowledgementDetailCode:_AcknowledgementDetailNotSupportedCode ;
        skos:definition  "The processing mode is not supported." ;
        skos:prefLabel   "Unsupported processing Mode" .

v3-AcknowledgementDetailCode:NS203
        a                owl:Class ;
        rdfs:label       "Unsupported version id" ;
        rdfs:subClassOf  v3-AcknowledgementDetailCode:_AcknowledgementDetailNotSupportedCode ;
        skos:definition  "The Version ID is not supported." ;
        skos:prefLabel   "Unsupported version id" .

v3-AcknowledgementDetailCode:SYN
        a                owl:Class ;
        rdfs:label       "Syntax error" ;
        skos:definition  "Reflects errors in the syntax or structure of the communication." ;
        skos:prefLabel   "Syntax error" .

v3-AcknowledgementDetailCode:INTERR
        a                owl:Class ;
        rdfs:label       "Internal system error" ;
        skos:definition  "An internal software component (database, application, queue mechanism, etc.) has failed, leading to inability to process the message." ;
        skos:prefLabel   "Internal system error" .

v3-AcknowledgementDetailCode:SYN105
        a                owl:Class ;
        rdfs:label       "Required element missing" ;
        rdfs:subClassOf  v3-AcknowledgementDetailCode:SYN ;
        skos:definition  "Description: Required association or attribute missing in message; or the sequence of the classes is different than required by the standard or one of the conformance profiles identified in the message." ;
        skos:prefLabel   "Required element missing" .

v3-AcknowledgementDetailCode:RTUDEST
        a                owl:Class ;
        rdfs:label       "Error: Message routing error, unknown destination." ;
        skos:definition  "The destination of this message is unknown to the receiving application. The receiving application in the message does not match the application which received the message. The message was neither routed, processed nor stored by the receiving application." ;
        skos:prefLabel   "Error: Message routing error, unknown destination." .

v3-AcknowledgementDetailCode:NS202
        a                owl:Class ;
        rdfs:label       "Unsupported processing id" ;
        rdfs:subClassOf  v3-AcknowledgementDetailCode:_AcknowledgementDetailNotSupportedCode ;
        skos:definition  "The Processing ID is not supported." ;
        skos:prefLabel   "Unsupported processing id" .

v3-AcknowledgementDetailCode:SYN114
        a                owl:Class ;
        rdfs:label       "Insufficient repetitions" ;
        rdfs:subClassOf  v3-AcknowledgementDetailCode:SYN105 ;
        skos:definition  "Description: The number of repetitions of a group of association or attributes is less than the required minimum for the standard or of one of the conformance profiles or templates identified in the message." ;
        skos:prefLabel   "Insufficient repetitions" .

v3-AcknowledgementDetailCode:SYN104
        a                owl:Class ;
        rdfs:label       "Invalid code system in CNE" ;
        rdfs:subClassOf  v3-AcknowledgementDetailCode:SYN106 ;
        skos:definition  "An attribute value referenced a code system that is not valid for an attribute constrained to CNE." ;
        skos:prefLabel   "Invalid code system in CNE" .

v3-AcknowledgementDetailCode:SYN113
        a                owl:Class ;
        rdfs:label       "Formal constraint violation" ;
        rdfs:subClassOf  v3-AcknowledgementDetailCode:SYN ;
        skos:definition  "Description: A formal constraint asserted in the standard or one of the conformance profiles or templates declared in the message has been violated." ;
        skos:prefLabel   "Formal constraint violation" .

v3-AcknowledgementDetailCode:SYN103
        a                owl:Class ;
        rdfs:label       "Value not found in code system" ;
        rdfs:subClassOf  v3-AcknowledgementDetailCode:SYN106 ;
        skos:definition  "An attribute value was compared against the corresponding code system, and no match was found." ;
        skos:prefLabel   "Value not found in code system" .

v3-AcknowledgementDetailCode:SYN109
        a                owl:Class ;
        rdfs:label       "Mandatory element with null value" ;
        rdfs:subClassOf  v3-AcknowledgementDetailCode:SYN ;
        skos:definition  "Description: An attribute or association identified as mandatory in a specification or declared conformance profile or template has been specified with a null flavor." ;
        skos:prefLabel   "Mandatory element with null value" .
